---
title: Adjunction
references: 
tags:
  - In_Progress
learning method: Vault + Read + Recall + Practice  (VRRP Method)
Current date: 2025-08-17
amount of time: 
learning score:
---
S
solve my equation exercise are equations that are given in the school broad 


![[Pasted image 20250817180611.png]] 


https://www.youtube.com/watch?v=a9nvXovb84Q 


$$
\begin{array}{l} 
(x + 3) (x+ 5)  (x + 7)(x + 9)   =  9   \\
(x^2  +8x + 15 ) (x^2 + 16x  + 63)  = 9  \\
x^4 +  16x^3  +  63x^2 + 8x^3 + 128x^2  +504x + 15x^2 + 240x + 945  = 9  \\
 x^4 + 24x^3 + 206x^2  +  744x + 936  =  0    \\
\text{ divide the equation by } x^2   \\
x^2 + 16x +  \frac{504}{x} + 15 +  \frac{240}{x}  +  \frac{936}{x^2}   =   0   
\end{array}


$$ 


$$
\begin{array}{l} 
(x + 3) (x+ 5)  (x + 7)(x + 9)   =  9   \\
\frac{3 + 5 + 7 + 9}{4} =  6  \\
(x  + 6  - 3 )( x + 6 -1)(x + 6 + 1) ( x + 6 + 3)   =  9   \\
\text{  y = x +  6}   \\
(y  - 3 )(y  -1)( y  + 1) ( y  + 3)   =  9   \\
(y^2 - 9)(y^2  -1)  =   9  \\
y^4  -y^2  - 9y^2  = 0  \\
y^4  - 10y^2  = 0  \\
y^2(y^2  - 10)  =  0  \\
\left\{ \begin{array}{l}
y^2  - 10  =   0  \\
y^2   =  0   \\
\end{array} \\
  \right.  \\
\left\{ \begin{array}{l}
(x +  6)^2    =   10   \\
(x +  6)^2   =  0   \\
\end{array} \\
  \right.  \\
\left\{ \begin{array}{l}
x  =   \pm \sqrt{ 10 }  -6  \\
x   =  -6   \\
\end{array} \\
  \right. 
\end{array}
$$






