---
title: Adjunction
references: https://www.youtube.com/watch?v=HfACrKJ_Y2w&ab_channel=freeCodeCamp.org
tags:
  - In_Progress
learning method: Vault + Read + Recall + Practice  (VRRP Method)
Current date: 2025-07-18
amount of time: 
learning score:
---


$$
\frac{21}{45} =  \frac{7\cdot  3} { 5 \cdot 3 \cdot 3}  =  \frac{7}{15}  
$$


simplify $\frac{3x  +  6} {x^2 + 4x + 4}$ 
$\frac{3(x  + 2)} {x + 2 }  = \frac{3}{x+ 2 }$ 
# multply and divding 

$$
\frac{4}{3}  \cdot \frac{2}{5 }   = \frac{2\cdot  4}{5 \cdot 3 }
$$


$$
\frac{\frac{4}{5}}{\frac{2}{3}}  =  \frac{4}{5}  \cdot \frac{3}{2}   = \frac{12}{10}  = \frac{6}{5 }
$$
compute   $$
\frac{\frac{x^2+ x }{x  + 4}}{\frac{x+1}{x^2 - 16}}  = 
$$



## adding and sub fraction 

used LCD 
$$
\frac{7}{6} - \frac{4}{15}  =  \frac{35 -  8}{30} =  \frac{27}{30 }  =  \frac{9}{10}
 $$
add
$$\frac{3}{2x+2}  +\frac{5}{x^2 -1}= \frac{3}{2(x  + 1 )} +  \frac{5}{(x + 1 )(x - 1)}  =  \frac{3x  - 3 +  10  }{2 (x + 1 ) (x - 1)}  =  \frac{3x + 7 }{2 (x + 1 ) (x - 1)}  $$
1. write both denominator in factor form  
2. multiply each denominator by the  missing factor  to have a common denominator using LCD logic 
3. do the add or addition operation 





# Different Quotient 

for function $y= f(x)$ 

## secant line is 
a line between two points on the slope of a function 

## definition the average rate of change for f(x) on the interval [a, b] is 
The secant line bteween the two point (a, f(a))  ) (b , f(b)) 
$$
 m=  \frac{rise}{ }  = \frac{y}{x }  = \frac{f(b) -f(a)}{b - a }
$$
Example the average rate of change for $f(x)  =\sqrt{ x }$ on the interval [1,4] is 
$$  
m = \frac{f(4)-f(1)}{4 -1 }   = \frac{\sqrt{ 4 } = \sqrt{ 1 }}{3} =
\frac{2-1}{3} = \frac{1}{3}
$$


A different quotation represent 
the average of change of a the function f(x ) on the intenal is [x, x + h] 


$$
m  =  \frac{f(b) -  f( c)}{ b -a }   = \frac{f(x+h)}{}
$$

the average rule 



example find the and simplify the different quitient for $f(x)= 2x^2  - x  + 3$
different   quotation  =  $\frac{f(x+h) - f(x)}{h}$ 

$$
\begin{array}
f(x+h) = 2(x+ h)^2  - (x + h) + 3   \\
2 (x+ h ) (x + h  )  - x  -h  + 3   \\
= 2(x^2 + x + h x + h^2 )  - x  - h  + 3  \\
= 2x^2 + 2xh + 2hx  + 2h^2 - x - h  + 3  \\
 =   2x^2 + 4xh + 2h^2 - x -h + 3 
\end{array}
$$
$$
\begin{array}
f(x+h) - f(x )   =    2x^2  = 4xh  + 2h^2  -x - h + 3 - (2x^2 -x + 3)  \\
= 2x^2 + 4xh  + 2h^2  -x -h + 3  - 2x^2  + x  - 3  \\

\end{array}

$$