1. find the vertical asympotes and horizontal asymptotes and holes 

horizontal asymptotes  :  

$$
\begin{array}{l} \\
q(x)  =  \frac{3x^2 + 3x} {2x^3 + 5x^2   - 3x } \\
 =  \frac{x^2}{ x^3}  = \frac{1}{x} \xrightarrow{\text{}}0 
\end{array}

$$


vertical asymptotes : 
$$
\begin{array}{l} \\
q(x)  =  \frac{3x^2 + 3x} {2x^3 + 5x^2   - 3x } \\
 =  \frac{3x(x + 1)}{x(2x^2 + 5x  - 3)}  = \frac{3(x + 1)}{(2x-1)(x + 3)} 
\end{array}
$$
$x=\frac{1}{2}\cap-3$ 


hole  : 
$$
 \frac{3(x + 1)}{(2x-1)(x + 3)}    = \frac{3(0 + 1)}{(2\cdot0-1)(0 + 3) }  = \frac{3}{-3}   = -1 
$$

(0,-1 )
find the verti