# #definition  

a rational expression is an expression where the numerator and denominator are polynomial 
## how to simply rational expression 

you can simplify rational expression by reducing them to the simplest fraction in the numerator and the denominator, then crossing the numbers that appear in both the numerator and denominator. finally multiply the tops and bottom again  
$$
\frac{21}{45} =  \frac{7\cdot  3} { 5 \cdot 3 \cdot 3}  =  \frac{7}{15}  
$$

this is also appliable to fraction with variables, where to top and the bottom can be reduce to the simples form  
$$\frac{3x  +  6} {x^2 + 4x + 4}=\frac{3(x  + 2)} {x + 2 }  = \frac{3}{x+ 2 }$$ 
here  I take out the common factor of the numerator then, crossing the numerator and the denominator out with the common term
# multiplying  and dividing   
multiplying factor between two faction only require you to common out multiply the numerator and denominator of the two rational expression 

$$
\frac{4}{3}  \cdot \frac{2}{5 }   = \frac{2\cdot  4}{5 \cdot 3 }
$$
dividing is flipping the the divided rational expression upside down then  do the same operation just like the multiplying factor  
$$
\frac{\frac{4}{5}}{\frac{2}{3}}  =  \frac{4}{5}  \cdot \frac{3}{2}   = \frac{12}{10}  = \frac{6}{5 }
$$
compute   $$
\frac{\frac{x^2+ x }{x  + 4}}{\frac{x+1}{x^2 - 16}}  = 
$$



## adding and sub fraction 

used LCD 
$$
\frac{7}{6} - \frac{4}{15}  =  \frac{35 -  8}{30} =  \frac{27}{30 }  =  \frac{9}{10}
 $$
add
$$\frac{3}{2x+2}  +\frac{5}{x^2 -1}= \frac{3}{2(x  + 1 )} +  \frac{5}{(x + 1 )(x - 1)}  =  \frac{3x  - 3 +  10  }{2 (x + 1 ) (x - 1)}  =  \frac{3x + 7 }{2 (x + 1 ) (x - 1)}  $$
1. write both denominator in factor form  
2. multiply each denominator by the  missing factor  to have a common denominator using LCD logic 
3. do the add or addition operation 

