https://www.wolframalpha.com/

$$ \begin{aligned} \wedge &= \text{and} \\ \lor &= \text{or} \\ \lnot &= \text{not} \end{aligned} $$ $$
\begin{aligned}
(m^{-7/3} n^{5/4})^{-8/9} &= m^{(-7/3) \cdot (-8/9)} n^{(5/4) \cdot (-8/9)} \\ &= m^{56/27} n^{-40/36}
\end{aligned}
$$

$$
\begin{aligned}
( \frac{a^{-1/3}  \cdot b^2 }{b^{2/3}  \cdot a^{-3/4}} )^{1/5} \\  & =  ( a^{-1/3}  \cdot b^2 \cdot b^{-2/3}  \cdot a^{3/4} )^{1/5} \\ &  = ( a^{5/12}  \cdot b^{4/3}   )^{1/5} \\ &  a^{1/12}  \cdot b^{4/15} 
\end{aligned}
$$



$$ 
\begin{aligned}
\left( \frac{p^{1/2} \cdot q^{1/3}}{p^{-1/3}\cdot q^{-1/4}} \right)^{-3}  \\&  = \left( \frac{1} { p^{-1/2} \cdot q^{-1/3} \cdot p^{-1/3} \cdot q^{-1/4}} \right)^{-3} \\&  = \left( \frac{1} { p^{-5/6} \cdot q^{-7/12}} \right)^{-3} \\&  =   \frac{1} { p^{5/18} \cdot q^{7/36}} 
\end{aligned}
$$

$$
\begin{aligned}
\left( \frac{a^2 b^{-4} c^{-1}}{b^{-9}c^{8}a^-4} \right)^{} \\ &= \left( \frac{c^{-9}}{b^{-5}a^{-6}} \right)^{-2}  \\ &=  \left( \frac{c^9}{ b^{5}a^{6}} \right)^{2}   \\ &=   \frac{c^{18}}{ b^{10}a^{12}} 
\end{aligned}
$$
$$
\begin{aligned}
(3x^{-2} y^{-4})^{-1} \\ & = \frac{x^2\cdot y^4}{3} 
\end{aligned}
$$

$$
\begin{aligned}
\frac{c^{-6}b^{10}}{b^9c^{-11}} \\ & =  c^{5}b^{1}
\end{aligned}
$$



$$
\begin{aligned}
\left(  \frac{ 4a^3(b^2a)^{-4}}{c^{-6}a^2 b^{-7}} \right) \\ & = \left(  \frac{ 4a^3\cdot b^{-8}\cdot a^{-4}}{c^{-6}a^2\cdot b^{-7}} \right) \\ &  = \left(  \frac{ 4\cdot c^{6} }{a^3\cdot b} \right)
\end{aligned}
$$


$$ 
\begin{aligned}
\left( \frac{(8x^{21})^0  y^{-3} x^8}{y^{-9} x ^{-1}}  \right)^6 \\ &  = \left( \frac{ y^{-3} x^8}{y^{-9} x ^{-1}}  \right)^6 \\ & =  \left(  y^{6} x^9  \right)^6 \\ &  =  y^{36} x^{54}
\end{aligned}
$$

$$
\begin{aligned}
\left(\frac{p^{-6}q^7\left(p^2q\right)^{-3}}{\left(p^{-1}q^{-4}\right)^2p^{10}}\right)^3   & \\   = 
\left(\frac{p^{-6}q^7 p^{-6}q^{-3} }{p^{-2}q^{-8}p^{10}}\right)^3   
& \\   = 
\left(\frac{q^{12} }{p^{20}}\right)^3   & \\   = \frac{q^{36} }{p^{60}}
\end{aligned} 
$$



$$
\begin{aligned}

\frac{\left(6v^2\right)^{-1}w^{-4}}{\left(2v\right)^{-3}w^{10}}   & \\  =   \frac{8v^{-2}w^{-4}}{6v^{-3}w^{10}}  & \\   =  \frac{8v}{6w^{6}}  
\end{aligned}
$$
  $$
  \begin{aligned}
\frac{4a^3(b^2a)^{-4}}{c^{-6}a^2b^{-7}}   & \\  =  \frac{4a^3 b^{-8}a^{-4}}{c^{-6}a^2b^{-7}}    & \\  = \frac{4c^{6} }{a^3b}
\end{aligned}
  $$
$$\left( \frac{c^{-6}b^{10}}{b^9c^{-11}} \right)  =  c^{5}b^{1} $$
$$



  \begin{aligned}
\left(\left(2a^2\right)^{-3}b^4\right)^{-3}  & \\   =  \left(\frac{a^{-6}b^4}{8}\right)^{-3}   & \\  =  \frac{a^{18}}{8b^{12}} 

\end{aligned}

$$

$$ 
 \begin{aligned}
\left( \frac{x^{3/4} y^{-2/3} }{x^{7/4}} \right)^{7/8} & \\   = \left( \frac{1  }{x\cdot y^{-2/3}} \right)^{7/8} & \\   = \left( \frac{1  }{x^{7/8}\cdot y^{7/12}} \right)

\end{aligned}
$$