---
title: Adjunction
references: https://tutorial.math.lamar.edu/Classes/CalcI/Functions.aspx
tags:
  - In_Progress
learning method: Vault + Read + Recall + Practice  (VRRP Method)
Current date: 2025-08-02
amount of time: 
learning score: 
reference: https://tutorial.math.lamar.edu/Solutions/CalcI/Functions/Prob2.aspx
---
Example 2 Given$f(x)=−x^2+6x−11$ find each of the following.



$$
\begin{array}{l} \\
f(x)=−x^2+6x−11      \\
f(2)=(−2)^2+6\cdot 2 −11    \\
 = 4 +  12  - 11   \\
  =  5     
\end{array}
$$

$$
\begin{array}{l} \\
f(x)=−x^2+6x−11      \\
f(2)=(−2)^2+6\cdot 2 −11    \\
 = 4 +  12  - 11   \\
  =  5     
\end{array}
$$



$$
\begin{array}{l} \\
 f(x)=−x^2+6x−11       \\
 f(4x  -1 ) =  -(4x  -1  )^2 +6(4x  - 1) −11    \\
  f(4x  -1 ) =   -16x^2  +8x   -1   +   24x  - 6   - 11   \\
   f(4x  -1 ) =   -16x^2  +  32x   -  18  
\end{array}
$$



## determine  all the roots of 
$$
f(t) =  9t^3    - 18t^2   +  6t   = 3t(3t^2  -  6t  + 2)      \implies 
\left\{\begin{array}{l}   \\
 t  =   0   \\
t = \frac{6^2  \pm \sqrt{ -6^2    -  4  \cdot  2 \cdot  }}{2 \cdot 3}  =  1 \mp  \frac{\sqrt{ 3 }}{3}
\end{array}
\right.




$$


## Find the domain and range of each of the following function 
$$
\begin{array}{l} \\
f(x )    =  5x  - 3    \\
\text{ the domain of this function is } (-\infty , \infty) \\
\text{ range of the function is }  (-\infty , \infty)
\end{array}
$$

$$
\begin{array}{l} \\
f(x )    = \sqrt{  4  - 7t }   \\
\text{ where }  t  \leq \frac{4}{7}
\text{ the domain of this function is } (-\infty , \frac{4}{7} ]   \\
\text{ range of the function is }  [0 , \infty)
\end{array}
$$ 

#fail 
$$
\begin{array}{l} \\
h (x)  =  -2x^2  + 12x +  5  \\
\text{  the domain of this function is} (-\infty , \infty)   \\
\text{ vertex  :} x = -\frac{12}{2 \cdot - 2 }    =3   +>(3,23) \\
\text{ range of the function is }  (-\infty , 23]
\end{array}
$$


$$
\begin{array}{l} \\
h (x)  = \mid  z - 6 \mid   - 3  \\
\text{  the domain of this function is} (-\infty , \infty)  \\
\text{ range of the function is }  [-3, \infty) 
\end{array}
$$

this is because the value  z - 6  cannot be less than 0 because of abs 

$$

\begin{array}{l} \\
g(x )  =  8 \\
\text{ the function have no domain }
\text{ range of the function is } 8
\end{array}
$$

## Find the domain of each of the following functions 

$$
\begin{array}{l} \\
f(x)  =  \frac{x  - 4}{x^2   - 2x  - 15}      \\
\text{ finding the domain }  \\
x^2   - 2x  - 15  = 0  \\
\left\{  \begin{array}{l}  
x= 5   \\
 x = -3 \\
\end{array}\right.    \\  \\
\text{ range of the function is } (-\infty  ,  -3 ) \cap ( -3 , 5)  \cap  (5 , \infty )    \\
\text{ range of the function is } (- \infty  ,\infty )
\end{array}
$$





$$
\begin{array}{l} \\
f(x)  = \sqrt{  6 + t - t^2 }     \\
\text{ finding the domain }  \\
 6 + t - t^2 \geq  0   \\
  t^2 - t -6   \leq  0   \\
\left\{  \begin{array}{l}  
t  =  -2   \\
t  = 3  
\end{array}\right.    \\  
\text{ domain of the function is } [-2  , 3 ]    \\
\end{array}
$$
I know that the function is negative or positive there because I plug in the number to see it 




$$
\begin{array}{l} \\
h (x) =   \frac{x}{\sqrt{ x^2 - 9  }} \\
\text{ finding the domain }  \\
x^2 - 9  >  0   \\

\left\{  \begin{array}{l}  
t  =  3   \\
t  = -3  
\end{array}\right.    \\  
\text{ domain of the function is } ( -\infty  ,   -3  ) \cap ( 3, \infty )    \\
\end{array}
$$
I know that the function is negative or positive there because I plug in the number to see it 


function composition :  F(x ) and g(x ) is 
given  $f(x) =3x^2-x + 10 \cap g(x) =1-20x$ find each of the following 
$$
\begin{array}{ l }   \\

(f∘g)(5)    \\
=  f(g(5))    \\
=  3(1  - 20 \cdot 5 )^2  -  (1  - 20 \cdot 5  )   +  10 \\
 = \\
(f∘g)(x) =  \\
(g∘f)(x)\\
(g∘g)(x)   \\
 =  g(g(  1 - 20x )  )  \\
=  1-20(1 - 20x )   \\
=   1 -  20  + 400x   \\
 = -19  + 400x  
\end{array}
$$

given $f(x)=3x - 2 \cap g(x) = \frac{1}{3}x+\frac{2}{3}$ 
$$
\begin{array}{ l }   \\

(f \circ  g) ( x)   \\
 = f(g(x))   \\
 = 3\left( \frac{1}{3}x + \frac{2}{3} \right)     -2   \\
 = x  +  2  - 2    \\
 = x   \\
(g \circ f) (x)   \\
= g(f(x)  )  \\
 =  \frac{1}{3}(3x-2)  +  \frac{2}{3 }     \\
 = x - \frac{2}{3}  + \frac{2}{3}  \\
 = x 
\end{array} 
$$



# #Practice_Exercise 

## For problems 1 – 4 the given functions perform the indicated function evaluations. 

 
 $$
\begin{array}{l}   \\  
f(x )  =  3 - 5x   -2x^2   \\
f(7  - 4x )  =  3 -  5( 7- 4x )   - 2(7- 4x)^2   \\
=  3 -  35 +  20x     -  2(49 + 16x^2  +  56x)  \\
= 3  - 35  + 20x  - 98 + 32x^2  + 112x   \\
=  \\
 \\

f(x + h)   \\
 =  3 - 5(x + h)   -2(x + h)^2  \\
= 3   - 5x  + h     -2 (x^2 + h^2  - 2xh)   \\
= 3 - 5x + h  - 2x^2  + 2h^2  - 4xh \\ 

\end{array}
$$


 $$
\begin{array}{l}  
g(t)  = \frac{t}{2t  + 6}   \\ 
g(t+ h) =  \frac{t +  h}{2 \cdot (t + h) + 6 }  \\
 =   \frac{t +  h}{2t + 2h + 6}   \\
g(t^2  - 3t  + 1)  =   \frac{t^2  - 3t  + 1}{2(t^2  - 3t  + 1)  + 6}     \\
 =   \frac{t^2  - 3t  + 1}{ 2t^2  - 6t  +  8  }
\end{array}
$$ 





 $$
\begin{array}{l}  
h(x)  =  \sqrt{ 1- z^2  }    \\
h(z^2  - 2z ) =   \sqrt{ 1-   (z^2  - 2z) }   \\
= \sqrt{ 1 - z^2   + 2z }  \\
h(z  +   k )  =  \sqrt{ 1- (z +  k)^2  }       \\
=  \sqrt{  1 - z^2   - k^2  -2kz  }
\end{array}
$$ 


## The **difference quotient** of a function f(x) is defined to be,  


$$
\begin{array}{l}
\frac{f(x + h )  - f(x)}{ h}        \\
f( x )  =  4x -  9 \implies   \frac{4(x  + h)  -  9  -  4x  - h  }{ h}   \\
 = \frac{4x  +  4h - 9  - 4x  - h } {  h}  \\
=   \frac{3h -9  } {  h}  
\end{array}

$$