---
title: Adjunction
references: https://tutorial.math.lamar.edu/Classes/Alg/Lines.aspx
tags:
  - In_Progress
learning method: Vault + Read + Recall + Practice  (VRRP Method)
Current date: "2025-08-17"
amount of time: 
learning score:
---
# #definition 

$$
\begin{array}{l} \\
\log_{2}(16 ) = \log_{2}2^4   =  4     \\
\log_{4} 16  =  \log_{4}4^2   = 2  \\
\log_{5} 625   =  \log_{5} 5^4  =  4 \\ 
\log_{9} \frac{1}{531441 }   = \log_{9} 9^{-5}   =-5    \\
\end{array}
$$

$$
\begin{array}{l} \\
\log_{\frac{1}{6} } 36   \\
 =   \log_{\frac{1}{6} }  6^2   \\
=  \log_{\frac{1}{6} }  \left( \frac{1}{6} \right)^{-2}   \\
 = -2
\end{array}
$$



$$
\begin{array}{l} \\
\log_{\frac{3}{2} }   = \log_{\frac{3}{2} }\left(  \frac{27}{8}  \right)  \\
=  \log_{\frac{3}{2} }\left( \frac{3}{2} \right)^3     \\
= 3  \\
\end{array}
$$






$$
\begin{array}{l} \\
\ln \sqrt[3]{ e }   =   \ln (e)^{1/3}    = \frac{1}{3} 
\end{array}
$$
$$
\log 1000  = \log 10^3    = 3   
$$

$$
\log_{16} 16  =1$$

$$
\log_{23} 1   = 0$$ 

$$
\log_{2} \sqrt[7]{32  } = \log_{2} 2^{5/7}   = \frac{5}{7}$$



## properties that are useful in the manipulation of logarithms. 


$$
\log_{3}\left( \frac{9x^4}{\sqrt{ y }} \right)  = \log_{3}(9x^4) -  \sqrt{ y }  =  \log_{3}(9) +   \log_{3}x^4  - \log_{3} \sqrt{ y }   =  2 +  4  \log_{3}x   - \frac{1}{2}\log_{3}  y
$$



# #Practice_Exercise 

$$
\begin{array}{l}
\log_{3}81   =  \log_{3}  3^4       =  4   \\
\log_{5}  125  = \log_{5} 5^3  = 3   \\
\log_{2} \frac{1}{8}  = -3   \\
\log_{\frac{1}{4} }  16  = \log{\frac{1}{4}} 4^2  = -2 
\end{array}

$$

## Write each of the following in terms of simpler logarithms. 




$$
\begin{array}{l}
\ln(x\sqrt{ y^2 + z^2 })  =  \ln x +  \frac{1}{2}\ln( y^2 + z^2)   \\
\end{array}
$$


$$
\begin{array}{l}
\log_{4} \frac{x-4}{y^2 \sqrt[5]{z  }}   \\
\log_{4}(x-4 )  -   \log_{4} y^2  +  \log_{4} \sqrt[5]{z  }   \\
\log_{4}(x-4 )  -   2\log_{4} y  +  \frac{5}{2}\log_{4} z   
\end{array}
$$

## Combine each of the following into a single logarithm with a coefficient of one. 




$$
\begin{array}{l}
2\log_{4} x  +  5\log_{4} y  - \frac{1}{2}\log_{4} z    \\
\log_{4} x^2    +  \log_{4} y^5   - \log_{4} \sqrt{ z }  \\
\log_{4} \left( \frac{x^2 y^5}{\sqrt{ z }}\right)
\end{array}
$$





$$
\begin{array}{l}
3\ln(t + 5 )   - 4 \ln t  -  2\ln(s  -1 )  \\
\ln (t + 5)^3  -  \ln  t^4 - \ln(s-1)^2      \\
\ln (t+ 5)^3  - (\ln t^4  +  \ln(s- 1)^2)   \\
\ln \frac{(t + 5)^3}{t^4 \cdot (s-1)^2}
\end{array}
$$
## Use the change of base formula and a calculator to find the value of each of the following. 


$$
\begin{array}{l}
\log_{12} 35  = \frac{ 35}{ }
\end{array}
$$





$$
\begin{array}{l}
3\ln(t + 5 )   - 4 \ln t  -  2\ln(s  -1 )  \\
\ln (t + 5)^3  -  \ln  t^4 - \ln(s-1)^2      \\
\ln (t+ 5)^3  - (\ln t^4  +  \ln(s- 1)^2)   \\
\ln \frac{(t + 5)^3}{t^4 \cdot (s-1)^2}
\end{array}
$$