---
title: Adjunction
references: https://tutorial.math.lamar.edu/Classes/CalcI/ExpLogEqns.aspx
tags:
  - In_Progress
learning method: Vault + Read + Recall + Practice  (VRRP Method)
Current date: 2025-08-18
amount of time: 
learning score:
---


$$
\begin{array}{l}  \\
7 +   15e^{1 -  3z}   = 10   \\
 \ln(15e^{1 -  3z} ) = \ln 3   \\
\ln(15)  +  \ln(e^{1 -  3z})  =  \ln 3   \\
1 -  3z  = -1.6094   \\
 z    = \frac{2.6094}{3} 
\end{array}
$$


$$
\begin{array}{l}  \\
10^{t^2  -t}   = 100   \\
t^2  -t   -2 =   0   \\
(t   - 2)(t  + 1 )  =    0   \\
\left\{ \begin{array}{l}  
t = 2   \\
t  = -1 
\end{array}  \right. 
  \end{array}
$$



$$
\begin{array}{l} \\
x -  xe^{5x + 2}  =   0  \\
x(1   -  e^{5x + 2})  =  0   \\
\left\{ \begin{array}{l} 
x = 0  \\
1  -  e^{5x + 2}  =   0   
\end{array} \right.   \\
\left\{ \begin{array}{l}  
x = 0  \\
x =  -\frac{2}{5 }  \\
\end{array} \right. 
\end{array}
$$





$$
\begin{array}{l} \\
 5(x^2  -  4)  = (x^2  - 4)  e^{ 7 - x}   \\
5(x^2 -4) -  (x^2  - 4)  e^{ 7 - x}       = 0   \\
(x^2  - 4)( 5  - e^{7-x})  =  0   \\
\left\{ \begin{array}{l} 
x^2  - 4 = 0  \\
 5  - e^{7-x}  =   0   
\end{array} \right.    \\
\left\{ \begin{array}{l} 
x  = \pm 2    \\
7-x  =   \ln 5   
\end{array} \right.    \\
\left\{ \begin{array}{l} 
x  = \pm 2    \\
x  =   -\ln 5 +7    
\end{array} \right.   \\
\end{array}
$$ 

$$
\begin{array}{l} \\
4e^{1 + 3x}  -  9e^{ 5-2x}  =  0   \\
\ln 4 e^{1 + 3x}     -  \ln 9e^{ 5-2x}     =0   \\
\ln 4 +    \ln e^{1 + 3x}  - \ln 9  -    \ln e^{ 5-2x}      = 0  \\
\ln 4 + 1 + 3x  - \ln 9  -  5 + 2x       =  0  \\
 5x   = 4.8109 \\
x  = 0.9621 \\
\end{array}
$$
another way of solving the equation : 
$$
 \begin{array}{l} \\
4e^{ 1 + 3x}  -  9e^{5 -2x}  =  0   \\
4e^{1  + 3 x  }    =   9e^{5   -2x}   \\
\frac{e^{1  + 3 x  }}{e^{5   -2x} }   =  \frac{9}{4}  \\
e^{   5 x   - 4  }  =    \frac{9}{4}    \\
 5x    =   \ln ( \frac{9}{4} )  +  4  \\
x   =0.9621 
\end{array}
$$
## some equations that involve logarithms. 
$$
b^{\log_{b} x   }  =   x  
$$


$$
\begin{array}{l} 
3 +  2 \ln\left( \frac{x}{7} +  3  \right)  =   -4  \\
\ln\left( \frac{x}{7} +  3  \right)    =   -\frac{7}{2}   \\
e^{\ln\left( \frac{x}{7} +  3  \right) }      = e^{-\frac{7}{2} }   \\
\frac{x}{7} +  3     =  e^{-\frac{7}{2} }   \\
x  = -20.7886 
 \end{array}
$$

##  one or more of the following properties to combine all the logarithms into a single logarithm. 
$$
\begin{array}{l} 
\log_{b}(xy)  = \log_{b}(x) + \log_{b}(y)   \\
\log_{b}\left( \frac{x}{y} \right)  = \log_{b}(x)  - \log_{b}(y)       \\
\log_{b}(x^{r})  = r\log_{b}(x)   
\end{array}
$$


$$
\begin{array}{l} \\
2\ln(\sqrt{ x } )   -  \ln(1 -x)  =2   \\
\ln\left( \frac{x}{1-x} \right)  = 2  \\
\frac{x}{1-x}  =  e^2   \\
x   =  e^2(1 -x )  \\
x =  e^2   - e^2x  \\
x  + e^2x  =  e^2   \\
x =   \frac{e^2}{(1 + e^2 )}
\end{array}
$$
ps : you should also check if the domain of the equation fit into the solution of this problem as well

$$
\begin{array}{l} \\
\log x   + \log(x - 3) =  1   \\
\log (x \cdot(x - 3))  =  1   \\
x^2  - 3x   - 10  = 0   \\
(x -  5)(x + 2 )  =  0  \\
\left\{ \begin{array}{l}  
x     =  5  \\
x = -2  
\end{array}  \right. 
\end{array}
$$

$$
 \begin{array}{l} \\
\ln(x - 2) + \ln(x  + 1 ) = 2   \\
\ln [(x - 2 )\cdot (x + 1)  ] =  2   \\
x^2   - x  - 2 - e^2     =     0   \\
\left\{ \begin{array}{l} 
x  = \frac{ 1  \pm \sqrt{ 1  -  4(-2  - e^2) } }{2} = \frac{ 1 \pm \sqrt{ 9 + 4e^2 }}{2}  \\
\end{array} \\  \right. 
 \\

\end{array}
$$


#todo 
create a script that read individual files in the md folder then combine it into 1 file with the name of the folder 


# #Practice_Exercise  

$$
 \begin{array}{l} \\
 \\12 -  4e^{ 7 + 3x}  =  7  \\
 -  4e^{ 7 + 3x}     = -5   \\
 e^{7 + 3x}   =   \frac{5}{4}    \\
7 + 3x   =  \ln \frac{5}{4}      \\
x =  −2.25895

\end{array}
$$


$$
 \begin{array}{l} \\
 1 =  10   -3e^{ z^2    -2z }  \\
e^{ z^2    -2z }   =  3   \\
z^2    -2z     -\ln 3  =    0   \\
\frac{-b \pm \sqrt{  b^2 -  4ac }}{2a}   \\
\frac{2\pm \sqrt{ 4 +  4\ln 3 }}{2}      \\
1\pm \sqrt{ 1+  1\ln 3 }
\end{array}
$$




$$
 \begin{array}{l} \\
2t  -  te^{6t - 1 }  =  0   \\
t(2   - e^{6t - 1 })   =0   \\
\left\{ \begin{array}{l} \\
 e^{6t - 1 }   = 2   \\
t =    0 
\end{array} \right.  \\
\left\{ \begin{array}{l} \\
6t - 1  = \ln 2  \\
t =    0 
\end{array} \right.    \\
\left\{ \begin{array}{l} \\
6t - 1  = \ln 2  \\
t =    0 
\end{array} \right.    
\end{array}
$$
