---
title: Adjunction
date: 2025-02-05
references: https://youtu.be/0EnklHkVKXI?feature=shared
tags:
  - In_Progress
reference:
---

# definition 
## what is factoring  
factoring is the process  of determining what what we multiple to get a given quantity  
$$
12 =  (2)(6)
$$
$$
12 = (-2)(-6)
$$
there are many other way to [[Factor]] 12 but these are the most common one 
## completely factorization 
the process of breaking down a factor to it prime number
$$
12 =  (2)(2)(3)
$$
## factoring polynomial  


factoring polynomial is the same process 
we continue to factor until we cannot get factor again  
$$
x^2  - 16 =  (x  + 4)(x-4)
$$
like wise this is not a complete factor 
$$
x^4 - 16  = (x^2 +14)(x^2 -14) 
$$
the complete factor of the above is  
$$
x^4  -16  =  (x^2 +4)(x+2)(x-2)
$$
# formula 
## greatest common factor
the best thing to do is used the greatest common factor try to see if there is a factor that is common to  all term  
$$
a(b+c) = ab+ac
$$
1. Common Factor  
	Example : 
	- 12 :  (**1**,12)  ,(**2**,6) , (3,**4**)  
	- 28 : (**1**,28) , (**2**,14) , (**4**, 7) 
	are factor that appear the most in two or more variables 
	Example : 
	- $12x^2:1,2,3,4,6,12,x,x^2$
	- $15x^4:1,3,5,15,x,x^2,x^3,x^4$ 
2. Greatest Common factors (Biggest Shared Factors)
	so in the first equation the greatest common factor is  4 
	in the second equation the greatest common factors is $3x^2$ 
## quick technique for factoring  

The diamond technique : 
 $ax^2 + bx +c$
 ![[6.2 Factorings 2025-02-05 15.42.40.excalidraw]] 
$(x+\# 1)(x+\#2)$   
$$
\begin{aligned}
\left\{\begin{array}{l}
if \; a  \; =   \;1 \to   do \; diamond \; factor  \\
a \; \neq  1   \to  do \; group \; factor 
\end{array} 
\right.

 
\end{aligned}
$$

what is the thing to check for if the first term polynomial 
- is it in order 
- is the first term positive  (help you to identify if you factor out a negative )
- factor out the GCF 
- then used the diamond method to factor and simplify even future 
proof   : 
$x^2 -13xy + 30y^2 =  x^2 -10xy - 3xy + 30y^2 = x(x-10y)-3y(x-10y)=(x -3y)(x-10y)$ 
![[Factoring  Polynomials 2025-02-06 12.35.58.excalidraw]]
- the  answer give us the correct  value for factoring 


## Perfect Square Trinomial (Sum Form)
$$
a^2+2ab+b^2=(a+b)^2
$$
## Perfect Square Trinomial (Difference Form) 
$$
a^2-2ab+b^2=(a-b)^2
$$
## Difference of Squares
$$
a^2-b^2=(a+b)(a-b)
$$
## Sum of Cubes
$$
a^3+b^3=(a+b)(a^2-ab+b^2)
$$
- the sum of cube and the different of cube have different sign  in the first and second parentheses  
## Difference of Cubes
$$
a^3-b^3=(a-b)(a^2+ab+b^2)
$$
- the sum of cube and the different of cube have different sign  in the first and second parentheses  
# practice exercise  




find the GCF  of : $-18y^{2},-63y^{3},27y^{4}$ 
1. start with the lowest number in the equations 
	-$18x^2$ :(1,18) ,(9,2) ,$y^2$
2. here we see that  9 is divided by 63 and 27 
3. so the GCF is $9y^2$ 
$49x -  35 = 7(7x-5)$ this used the [[Factoring  Polynomials#greatest common factor]]  7 
 find the GCF of :   $5x^2y^4(2n+n)-(2n+n)$  
4. we can see that the right and left equation separated by a negative sign  
5. we can see there is a common factor (2n+n) 
6. se we will factor out (2n+n) in the term we will get 
	$(2n+n)(5x^2y^4-1)$
find the GCF of :  $xy + 2x + 3y +6$ 
1. first we will get rid of the common factor on the two equation from the left and right 
	$x(y+2)+3(y+2)$
2. then we will put the common factor (y + 2 ) out of the term 
	$(y+2)+(x+3)$
find the GCF of :  $3a^2 +4ab +3a+4b$ 
3.  first we will switch the position of 4ab and 3a 
	$3a^2+3a +4ab +4b$  
4. then we will get rid of the common factor on the two equation from the left and right  
	$3a(a + 1) + 4b(a+1)$  
5. then we will  put the (a+1 ) out of the term 
	$(a+1)(3a + 4b)$  




## factoring  quadratic polynomials 

$$
4x^2   +10x  -6 =  (2x-1)(2x+6)
$$
### Factoring Polynomials (a =1)

$$
x^2  +6x-  9    =  (x+3)(x+3)  = (x+3)^2
$$


## different of square factoring 
1. are the terms in order 
2. is the first terms positive 
3. is there a GCF 
4. then count the number of terms 
$a^2  - b^2 = (a+b)  (a-b)$   
Exercise : 
$x^2  - 16 =  x^2 - 4^2 = (x- 4)  (x + 4)$ 
1. yes 
2. yes  
3. no  
4. the numbers of terms is 2 
$y^2  + 64  \neq$ 
1. no  
2. yes  
3. no  
4. the numbers of terms is 2 
$\to$  there  is no way to do the diamond problem 
$y^2  - \frac{25}{81} = y^2   -  \left(  \frac{5}{9} \right)^2 = (y- \frac{5}{9} )  (y+ \frac{5}{9})$ 
1. yes 
2. yes  
3. no  
4. the numbers of terms is 2 
$9y^3-25y =  y(9y^2-25)  =  y(3y-5)(3y+5)$  
1. yes 
2. yes  
3. yes 
4. the numbers of terms is 2 
$80y^4-5 =  5(16y^4 - 1  )  =  5(4y^2-1)(4y^2+1)$    
1. yes 
2. yes  
3. yes 
4. the numbers of terms is 2 



###  factoring  quadratic polynomials  with  GCF 

what is the thing to check for if the first term polynomial 
- is it in order 
- is the first term positive  (help you to identify if you factor out a negative )
- factor out the GCF 
- then used the diamond method to factor and simplify even future 
$5x^5 - 25x^4 - 30x^3$ =  $5x^3[x^2 - 5x - 6]$ =   $5x^3(x-6)(x+1)$ 
$$
3.x^4  -  3.x^3  - 36x^2  =  3x^2(X^2  - X - 12)   =  3X^2(x-4).(x+3)

$$
## factoring   Â Quadratic Polynomials  with greater than 2 degree 



solving this equation by using the [[Factoring  Polynomials#Difference of Squares]]
$$
x^4  - 25  =  (x^2+5)(x^2-5)
$$
$$
x^4  +  x^2 -20 = (x^2-4)(x^2 +5)   =  
(x-2)(x+2)(x^2 + 5)
$$ 

### Factoring Polynomials (Trinomials) in General

Exercise : 
 $$ 
 \begin{array}{l}
2x^2   +13x  -7    \\
=2x^2   -1x + 14x   -7  \\
 =x(2x -1) + 7(2x -1)  \\ 
 =(x +7)(2x -1)  \\
\end{array}
 $$


$$

$$
![[6.2 Factorings 2025-02-05 16.14.11.excalidraw]] 

 $$ 
 \begin{array}{l}
8x^2   -22x  +5    \\
 =2x(4x -1) - 5(4x -1)  \\ 
 =(2x -5)(4x -1)  \\
\end{array}
 $$
![[6.2 Factorings 2025-02-05 16.21.50.excalidraw]]



Factoring  the greatest common division before using the diamond method : 
 $$ 
 \begin{array}{l}
6xy^2   +33xy  -18x    \\
 =3x[2y^2   +11y  -6    ]  \\
 =3x[2y^2  +12y - y  - 6    ] \\
 =3x[2y(y+6) -(y+6)    ]  \\
 =3x(y+6) (2y-1) 
\end{array}
 $$
 ![[6.2 Factorings 2025-02-05 16.24.19.excalidraw]]
factoring using the diamond method does not have to be $x^2 , x$  
$$
\begin{array}{l} \\
25x^4  - 20x + 4 \\
=25x^4  - 10x^2  - 10x^2 + 4  \\  
= 5x^2(5x^2 -2) -2(5x^2 -2)   \\
= (5x^2 -2)(5x^2 -2)  \\
= (5x^2 -2)^2
\end{array}
$$

![[6.2 Factorings 2025-02-05 16.39.55.excalidraw]]  


## solving factor  polynomials 
$$
\begin{array}
 & y^2 -3y  -18 =  0   \\
(y-6)(y+3)  =   0  
\end{array}
$$

$$


\left\{
\begin{array}{l}
y  -  6 = 0  \\
y + 3 = 0   \\

\end{array}
\right.
\implies
\left\{
\begin{array}{l}
y  = 6 \\
y =  - 3  \\

\end{array}
\right.

$$  


$$
\begin{array}
 & y^2 + 5y  + 6  =  0   \\
(y+3)(y+2)  =   0  
\end{array}
$$

$$


\left\{
\begin{array}{l}
y  + 2 = 0  \\
y + 3 = 0   \\

\end{array}
\right.
\implies
\left\{
\begin{array}{l}
y  = -2 \\
y =  - 3  \\

\end{array}
\right.

$$  



$$
\begin{array}
 & 25y^2 - 29y  + 4  =  0    
 \\ 25y(y-1)-4y(y-1) =    0   \\
(25y-4y)(y-1) =    0  \\


\end{array}
$$

$$


\left\{
\begin{array}{l}
y  -1  = 0  \\
25y  - 4 = 0   \\

\end{array}
\right.
\implies
\left\{
\begin{array}{l}
y  = 1 \\
y =  \frac{4}{25}  \\

\end{array}
\right.

$$  




$$
\begin{array}
 & y(y -4 ) =  5      
 \\  y(y -4 )     - 5 =    0   \\
y^2 -  4y      - 5 =    0  \\ 
(y - 5)(y +1) =   0  \\


\end{array}
$$

$$


\left\{
\begin{array}{l}
y  + 1  = 0  \\
y-5  = 0   \\

\end{array}
\right.
\implies
\left\{
\begin{array}{l}
y  =  - 1 \\
y =  5  \\

\end{array}
\right.

$$




$$
\begin{array}
 & (3y - 2 ) ( 2y^2    -13 y  + 15 ) =  0    
 \\ (3y - 2 ) (y+1) ( 2y  -15 )   =    0   \\


\end{array}
$$

$$


\left\{
\begin{array}{l}
3y  -2  = 0  \\
2y - 15  = 0   \\
y  +1  = 0  \\

\end{array}
\right.
\implies
\left\{
\begin{array}{l}
y   = \frac{2}{3}  \\
y   = -1  \\
y   = \frac{15}{2}  \\
\end{array}
\right.

$$  

