---
title: Adjunction
date: 2024-12-07
references: 
tags:
  - In_Progress
reference:
---
# #Definition  
rational  expression , is a  fraction which have the numerator and the  denominator  as a  polynomial
A FRACTION WHERE BOTH THE NUMER AND DENOM. ARE  POLYNOMIALS  

$$\frac{P}{Q}$$
here are some basic example : 
$\frac{6}{x-1}$
$\frac{z^2  -1}{z^2 +5}$ 
$\frac{z^2  -1}{1}$ 


- this is a rational  function  
- you can never divide by 0  in a rational function 
the last equation seem to be strange, but the important thing to note is that a polynomials expression can be  thought of as a rational expressions if we need to    
 
Note : for any rational function the denominator   cannot be zero   
if the denominator is zero at some point then the function is zero at that point 
it okay for a numerator to equal to zero 

$$
f(x) =  \frac{x^2   + 1  }{x-6}
$$
find domains  : number  
$$


\{\begin{array}{l}
x |  is \;  A \; real \; number  \cap x \neq 6 
\end{array}


$$
- not okey due to the rule the denominator is not a real number 
- $x - 6  \neq 0 \implies x   = 6$ 
To Find Domain  , Set Denominator $\neq$ 0 


$G(x) = \frac{x^2+ 9}{4}$
$$


\{\begin{array}{l}
x |  is \;  A \; real \; number    
\end{array}


$$

$$h(x) =  \frac{5x^2 + 9}{x+ 2}$$$$
\{\begin{array}{l}
x |  is \;  A \; real \; number   \cap x \neq -2  
\end{array}
$$- $x + 2  \neq 0 \implies x   = -2$



$$f(x) =  \frac{5x + 4}{x^2 - 3x - 10}$$ 

$$
\{\begin{array}{l}
x |  is \;  A \; real \; number    \cap x \neq 5   , x  \neq -2 
\end{array}
$$ $x^2 - 3x - 10   \neq 0$  
![[Rational Function 2025-02-07 17.29.18.excalidraw]] 
$$
\begin{aligned}
(x-5)(x+ 2 )\neq 0  \\
\{\begin{array}{l}
x-5 \neq 0   \\
x+ 2 \neq 0  \\

\end{array} 
\{\begin{array}{l}
x \neq5\\
x \neq - 2 \\

\end{array}
\end{aligned}

$$ 
## exception  

when dealing with rational expression  we will always assume that  the denominator $\neq$ 0  

### property of negative fractions
the following are all equivalent  
$$-\frac{a}{b}=\frac{-a}{b^{\bullet}}=\frac{a}{-b}$$
the following are all equivalent , the negative notation on x cannot be factor out of the numerator due to it only being attach to x . In order to  move the negative notation  we much time the numerator by x then shift the negative notation   
$$\frac{-x+3}{x+1}=\frac{-(x-3)}{x+1}=-\frac{x-3}{x+1}$$
## #simplified Rational Expression 

A Rational Expression has been reduce to it lowest terms if all common [[Factor]]s from the numerator and the denominator have been canceled 


## common denominator 
In order for a subtraction  and addition for rational expression  to take place , there much be a common denominator. 

$$\frac{a}{c}+\frac{b}{c}=\frac{a+b}{c} \; \frac{a}{c}-\frac{b}{c}=\frac{a-b}{c}$$

The most suitable choice for a common denominator is the least common  denominator 
example : 
$$\frac{5}{6}-\frac{3}{4}=\frac{5\left(2\right)}{6\left(2\right)}-\frac{3\left(3\right)}{4\left(3\right)}=\frac{10}{12}-\frac{9}{12}=\frac{10-9}{12}=\frac{1}{12}$$
- here we will multiply the left factorial  2 and the right by 3 creating  a common denominator of  12 
finding the least common denominator in a rational expression you need to follow these step 
example : 
$$\frac{4}{6x^2}-\frac{1}{3x^5}+\frac{5}{2x^3}$$
1. reduce the all the  denominator to it factors  
	- $$\frac{4}{3.2x^2}-\frac{1}{3x^5}+\frac{5}{2x^3}$$
2. write down  all the factor that appear at least one , do not write down the  power of a factors 
	- the unique factors that appear is  3,2,x 
3. now for every  coefficient write down it largest power in this cases the coefficient of x have the largest power of 5 
4. the product of all the factors in the previous step is the lcd which is $6x^5$
#  practice exercise
## simplify  
$$
\frac{x^2 - 2x - 8}{x^2 - 9x +20} =  \frac{(x-4)(x+2)}{(x-4)(x-5)}   =\frac{x+2}{x-5}  
$$

[[Factoring  Polynomials#Difference of Squares]]
$$
\frac{x^2  - 25}{(5x-x^2)} =  \frac{(x - 5)(x+5)}{-x(x-5)} =  \frac{x+5}{-x}
$$

[[Factoring  Polynomials#Perfect Square Trinomial (Sum Form)]]
$$
\frac{x^7   + 2x^6  + x^5}{x^3 (x+1)}  = \frac{x^5(x^2+2x + 1)}{x^3(x+1)^8} = \frac{x^5.(x+1)^2}{x^3(x+1)^8} = \frac{x^2}{(x+1)^6}
$$

$$
\begin{array}{l}
\frac{5}{17}  \\
\frac{6}{18} 
\end{array} 
$$
simplify when the denominator and  numerator is similar have common value 
Faction 

$$\frac{15}{35}  =  \frac{5\cdot 3}{ 5\cdot 7 }  = \frac{5}{  5 } \cdot \frac{3}{  7   }  = \frac{3}{7}$$

the first thing  you need to do before  common factor you need to know factoring  
$$
\begin{array}{l}
\frac{(x+2)^2}{x^2 - 4}  \\
=\frac{(x+2)^2}{x^2 - 2^2}  \\
=\frac{(x+2)^2}{(x-2 )(x+ 2)} \\
=\frac{(x+2)}{(x-2 )} \\
\end{array} $$
$$ \begin{array}{l}
\frac{3y^3}{6y^4  - 3y^3}  \\
 = \frac{3y^3}{3y^3 (2y -1)} \\
= \frac{1}{2y - 1}
\end{array}
$$

$$
\frac{5x^2 -6x + 1}{ 3x^2 + 4x- 7} 
$$

![[7.1 Rational Function 2025-02-10 13.20.34.excalidraw]]

![[7.1 Rational Function 2025-02-10 13.21.00.excalidraw]]
$$ 
\begin{array}{l}
\frac{5x^2 -6x + 1}{ 3x^2 + 4x- 7}    \\
 = \frac{5x^2 -6x + 1}{ 3x^2 + 4x- 7}  \\
 = \frac{(3x + 7)(x -1 )}{ ( 5x- 1)(x -1 )}  \\
 = \frac{(3x + 7)}{ ( 5x- 1)}
\end{array} 

$$

$$ 
\begin{array}{l}
\frac{5x^4}{ 10x^5  -  5z^3 }    \\
 = \frac{5x^4}{ 5x^3\cdot(2x^2 - 1 ) }   \\
 = \frac{x}{ 2x^2 - 1 }  \\
\end{array} 

$$
Factor  to make the term with the largest exponent positive   
Step: 
1. Factor both numerator and denominator completely    
2. Simplify  Common factor , not common terms  
HTTP://sites.google.com/site/professorleon57  for home work 
$$
\begin{array}{l} 
\frac{20-5x^2}{x^2 + x - 6}   \\
= \frac{-5(-4 + x^2)}{(x+3)(x - 2)}   \\
 = \frac{-5(x^2 - 4)}{(x+3)(x - 2)}   \\
 = \frac{-5\cdot(x - 2 ) (x+ 2)}{(x+3)(x - 2)}   \\
 = \frac{-5(x+ 2)}{(x+3)} 
\end{array} 

$$


$$
\begin{array}{l}
\frac{9x^5  - 3x^4}{ 3x^3}  \\
=\frac{3x^3(3x^2  - 1x)}{ 3x^3 }  \\   \\
= 3x^2  - x 
\end{array}
$$ 



$$
\begin{array}{l}
\frac{3 -  3x^2}{ x^2 + x - 2}  \\
=\frac{-3( x^2  - 1)}{ (x  + 2 ) (x -1) }  \\   
=\frac{-3(x -1) (x+ 1)}{ (x  + 2 ) (x -1) } \\
=\frac{  -3(x+ 1 )}{ x+ 2} 
\end{array}
$$
![[7.1 Rational Function 2025-02-10 13.51.54.excalidraw]]  


$$
\begin{array}{l}   \\
 = \frac{x^3+ 27}{x + 3}   \\ 
 = \frac{(x + 3)(x^2  - 3x +   9 )}{x + 3}  \\
  = (x^2  - 3x +   9 )
\end{array}
$$

=$$
\begin{array}{l}   \\
 = \frac{3x^2 + 5}{x^3  -3x^2 +2x  - 6}   \\ 
 = \frac{(x + 3)(x^2  - 3x +   9 )}{x + 3}  \\
  = (x^2  - 3x +   9 )
\end{array}
$$