

# #definition  
The  tittle  of this exercise suggest   that we will be  solving  radicals equation . But for added challenge   we will be  presenting them as  a square root  .  Spare Root  cause the equation  to  be must more messier  
This is similar to section  [[Section 2.9  Equations Reducible to Quadratic in Form]]  . However,  even though the approach may be the same ,  the application needs  to  be applied  differ  .
Here is an example 
$$
\begin{array}{l}
x =   \sqrt{ x +  6   }   \\

\end{array}
$$
Notice that if we square both size the square root will go always   
$$
\begin{array}{l}
x =   \sqrt{ x +  6   }   \\
x^2  =   x+ 6   \\
x^2   - x -   6    = 0  \\
(x  -  3) ( x  +  2 )     =   0   \\
\left\{
\begin{array}{l}
  x  =  3  \\
x  = -2 \\
 
\end{array} \\

\right.  
\end{array}
$$
Now  let do something different ,  we will now check the answer    of the above equation  
$$\begin{aligned}&3\overset{?}{\operatorname*{\operatorname*{=}}}\sqrt{3+6}\\&3=\sqrt{9}&\mathrm{OK}\end{aligned}$$ So  x =  3  is a solution ,  what about  x   =  -2 
$$
\begin{aligned}&-2\overset{?}{\operatorname*{\operatorname*{=}}}\sqrt{-2+6}\\&-2\neq\sqrt{4}=2&\mathrm{NOT~OK}\end{aligned}
$$

we have a problem recall that latex always   be positive  ,  and so    $x    =  -2$  does not wo rk  in the original  equation  .  Remember that the first step  to  solve  this equation  is to square both side , so if  we plug  in the value -2  the  solution  will work  with  that  equation .  So in conclusion  ,   the equation  that we started  out with and the equation we  change to solve the problem are different so  we should expect valid  and  un valid result  
##  more couple of example 

$$\begin{array}{l}
y   +  \sqrt{ y -4 }  =   4  \\
y    -  4 =   \sqrt{   y  - 4 }   \\
(y -4 )^2     =   y -4   \\
y^2  -   8y  + 16  =   y  -  4   \\
y^2  -  9y  +  20    =  0   \\
(y  -  4)  ( y   -5)   = 0    \\
\left\{
\begin{array}{l}
  y  =  4 \\
y  = 5 \\
 
\end{array} \\
\implies   \\
\left\{
\begin{array}{l}
  y  =  4 \\
y  = 5 \\

\end{array} 
\right. 
\right. 
\end{array}$$
only   y   =  4 satisfy the solution since   $4   +  \sqrt{ 4 -4 }  =   4$  


#fail  

$$\begin{array}{l}
1  =    t +   \sqrt{  2t  - 3   }  \\ 
1   -  t  =       \sqrt{  2t  - 3   }    \\
(1   -  t)^2   =  2t  - 3   \\
t^2  -      2t   + 1        =  2t  - 3   \\
t^2   - 4t  + 4    = 0    \\
t   =   \frac{4  \pm    \sqrt{  16  -4\cdot 4 \cdot 1 }}{2} \\
\left\{
\begin{array}{l}
  y  = 2    \\
y  = 2   \\ 
 
\end{array} \\
 
\right. 
\end{array}$$




#fail 

$$\begin{array}{l}
\sqrt{ 5z  +  6 }  -2  =  z     \\
\sqrt{ 5z  +  6 }      = z   + 2   \\
5z   +  6   =   (z  + 2)^2  \\
5z  +  6  =  z^2   + 4z  + 4   \\
-z^2  + z   + 2   = 0    \\
z^2  - z  - 2  =     0    \\  
( z    -     2)(z   +  1 )  =  0     \\

\left\{
\begin{array}{l}
 z    -     2    = 0    \\
z   +  1    =0   \\ 
 
\end{array} \\
\implies  \\  \\
\left\{
\begin{array}{l}
 z     = +2  \\
z       =-1    \\ 
 
\end{array} \\ 
\right. 
\right. 
\end{array}$$ 

the only solution to this  problem  is  -1  

## Solution with  more than one square root 
all the solution that we have look at have   only one square root . But not ,  let look  at different problem  with  square root  larger  then  one    
Solve each of the following equation  
#fail  
$$
\begin{array}{l}   \\
\sqrt{ 2x   - 1    }   -   \sqrt{  x  - 4 }  =  2    \\
\sqrt{ 2x   - 1    }      =  2  +  \sqrt{  x  - 4 }    \\
2x    -  1   =   (2  +  \sqrt{  x  - 4 } )(2  +  \sqrt{  x  - 4 } )  \\
2x    -  1   =   4  +  2 \sqrt{  x  - 4 }  + 2 \sqrt{  x  - 4 }  + (  x  - 4 )    \\
2x    -  1   =   4  +  4 \sqrt{  x  - 4 }   +  x  - 4   \\
x    -  1    =  4 \sqrt{  x  - 4 }    \\
(x  - 1 )^2  =    16 (x  - 4 ) \\
x^2   -2x   + 1   =    16x  -        \\
 \left\{
\begin{array}{l}
 z    -     2    = 0    \\
z   +  1    =0   \\ 
 
\end{array} \\
\implies  \\  \\
\left\{
\begin{array}{l}
 z     = +2  \\
z       =-1    \\ 
 
\end{array} \\ 
\right. 
\right. 
\end{array}
$$