
# #definition   
we going to  be look  at equation  that when  in  the correct light can turn  into quadratic  equation . 
$$
\begin{array}{l}
x^4   -  7x^2  +  12     \\
(x^2)^2   - (7x)^2  + 12    \\
u   =  x^2   \\
\implies  u^2   - 7u^2  + 12 =0   \\
( u  -3 ) ( u -4 )    \\
 \left\{
\begin{array}{l}
  u  =   3    \\
u  = 4   \\
 
\end{array} \\
\implies
\left\{
\begin{array}{l}
  x^2   =   3    \\
x^2  = 4   \\
 

\end{array}
\right. \\
\implies
\left\{
\begin{array}{l}
  x  = \pm  \sqrt{ 3 }    \\
x =  \pm 2   \\
 

\end{array}
\right.
\right.  
 \end{array}
$$
the basic process    is to check that the equation    is reducible  to quadratic in form then  make quick   substitution  to turn it into a quadratic equation  . Here we  solve the variable  u  used for  substituting   $x^2$  then  solve  $x^2$  bases on  the variable  

## solve each of the following  equation  




$$
\begin{array}{l}
 x^{2/3} - 2x^{1/3} - 15  =  0  \\
u  = x^{\frac{1}{3} }    \\
 \implies u^2      -  2u  -  15   =    0    \\
(u   + 3) (  u   - 5  )   =   0   \\
 \left\{
\begin{array}{l}
  u  =   -3    \\
u  = 5   \\
 
\end{array} \\
\implies
\left\{
\begin{array}{l}
x^{\frac{1}{3} }     =  -3     \\
x^{\frac{1}{3} }   = 5   \\
 

\end{array}
\right. \\
\implies
\left\{
\begin{array}{l}
x   =  (-3)^3    =  -27    \\
x   = (5)^3  =  125 
 

\end{array}
\right.
\right.  
 \end{array}
$$ 
#fail 
$$
\begin{array}{l}
y^{−6}−9y^{−3}+8=0 \\
u  = y^{−3}     \\
 \implies u^2      -  9u  +   8     =    0    \\
(u   -1   ) (  u   -   8    )   =   0   \\
 \left\{
\begin{array}{l}
  u  =   1    \\
u  =  8    \\
 
\end{array} \\
\implies
\left\{
\begin{array}{l}
y^{−3}     =  1    \\
y^{−3}    =  8    \\
 

\end{array}
\right. \\
\implies
\left\{
\begin{array}{l}
 y    =    1      \\
x   =    \frac{1}{ 2} 
 

\end{array}
\right.
\right.  
 \end{array}
$$



$$
\begin{array}{l}
z−9\sqrt{  z  }+14=0 \\
u  = z^{1/2}   \\
 \implies u^2−9u+14=0     \\
(u    -   2 ) (  u     -  7  )   =   0   \\
 \left\{
\begin{array}{l}
  u  =   2    \\
u  = 7  \\
 
\end{array} \\
\implies
\left\{
\begin{array}{l}
 z^{1/2}     =  2     \\
 z^{1/2}    = 7    \\
\end{array}
\right. \\
\implies
\left\{
\begin{array}{l}
x   =  4   \\
x   =   49      
 

\end{array}
\right.
\right.  
 \end{array}
$$ 



$$
\begin{array}{l}
t^4−4=0\\
 u =   t^2     \\
 \implies u^2   - 4  =    0      \\
(u-2) (  u + 2  )   =   0   \\
 \left\{
\begin{array}{l}
  u  =   2    \\
u  =  - 2    \\
 
\end{array} \\
\implies
\left\{
\begin{array}{l}
 t^2   =   2    \\
t^2    =  - 2    \\
\end{array}
\right. \\
\implies
\left\{
\begin{array}{l}
t   =   \pm   \sqrt{   2 }  \\
t    =    \pm   \sqrt{  2 } \cdot i 
 

\end{array}
\right.
\right.  
 \end{array}
$$



$$
\begin{array}{l}
2x^{10}−x^5−4=0\\
 u =   x^5    \\
 \implies 2u^2   -  u   -  4   =    0      \\
  =\frac{  1  \pm   \sqrt{ 1  - 4\cdot 2 \cdot   -4}}{ 4  }  \\
 =  \frac{  1  \pm   \sqrt{33}}{ 4  } 
 \left\{
\begin{array}{l}
  u  =  \frac{  1   +   \sqrt{33}}{ 4  }     \\
u  =  \frac{  1  -    \sqrt{33}}{ 4  }    \\
 
\end{array} \\
\implies
\left\{
\begin{array}{l}
x^5  =  \frac{  1   +   \sqrt{33}}{ 4  }    \\
x^5    =  \frac{  1  -    \sqrt{33}}{ 4  }      \\
\end{array}
\right. \\
\implies
\left\{
\begin{array}{l}
x  =  \left( \frac{  1   +   \sqrt{33}}{ 4  }  \right)^{1/5}   \\
x   =  \left( \frac{  1  -    \sqrt{33}}{ 4  } \right)^{1/5}      \\
 

\end{array}
\right.
\right.  
 \end{array}
$$




# #Practice_Exercise  

## Solve each of the following equations.  

$$
\begin{array}{l}
x^6−9x^3+8=0  \\ 
 u =   x^3 \\
 \implies u^2   -  9u    +   8  =    0      \\
 (u  -  1) ( u   -   8  )   \\

 \left\{
\begin{array}{l}
  u  = 1    \\
u  =  8    \\
 
\end{array} \\
\implies
\left\{
\begin{array}{l}
   x^3  = 1    \\
 x^3  =  8    \\
\end{array}
\right. \\
\implies
\left\{
\begin{array}{l}
x  =  1  \\
x   = 2    \\
 

\end{array}
\right.
\right.  
 \end{array}
$$  


$$
\begin{array}{l}
x^{−4}−7x^{−2}−18=0  \\ 
 u =   x^{-2 } \\
 \implies  u^2  −7u−18=0        \\
(   u  -  9) (  u  + 2  )  \\

 \left\{
\begin{array}{l}
  u  = 9    \\
u  =      -2   \\
 
\end{array} \\
\implies
\left\{
\begin{array}{l}
x^{-2 }  = 9    \\
x^{-2 } =      -2   \\
\end{array}
\right. \\
\implies
\left\{
\begin{array}{l}
x  =  \frac{1}{}  \\
x   = 2    \\
 

\end{array}
\right.
\right.  
 \end{array}
$$