---
title: Adjunction
references: 
tags:
  - In_Progress
reference: 
Current date: "2025-03-12"
---

# #definition  
We' ll start off the solving portion of the chapter by   solving a linear equation ,  a linear equation is any equation that is written  in the form  : 
$$ax +  b  =  0$$ where a and b  is a real number and x  is a variable  . This is the standard form of a linear equation  . Note that most linear equation do not start of with form   .Also  , the variable are not always x so do not assume x for every linear equation 

$a=b$ then $a+ c   =  b + c$ this is all  to say that we can add c to each side of the equation 
$a=b$ then $a- c   =  b + c$ this is all  to say that we can subject  c to each side of the equation 
$a=b$ then $a\cdot c  =  b\cdot c$ this is all  to say that we can multiply c to each side of the equation 
a = b then $\frac{a}{c}  =\frac{b}{c}$ for nay non-zero c . We can divided  both side  of an equation  by a non-zero number . c without changing the equation 
One way to thing of these rule is that . What we do to one side  of the equation we will do to the other side of the equation 


# Process for solving Linear Equation  
1. If the equation contains any fractions use the least common denominator to clear the fractions. We will do this by multiplying both sides of the equation by the LCD.  
      
    Also, if there are variables in the denominators of the fractions identify values of the variable which will give division by zero as we will need to avoid these values in our solution.  
      
    
2. Simplify both sides of the equation. This means clearing out any parenthesis and combining like terms.  
      
    
3. Use the first two facts above to get all terms with the variable in them on one side of the equations (combining into a single term of course) and all constants on the other side.  
      
    
4. If the coefficient (definition of coefficient is in [[Polynomials]] ) of the variable is not a one use the  third or fourth  method in the #definition   above (this will depend on just what the number is) to make the coefficient a one.  
      
    Note that we usually just divide both sides of the equation by the coefficient if it is an integer or multiply both sides of the equation by the reciprocal of the coefficient if it is a fraction.  
      
    
5. **VERIFY YOUR ANSWER!** This is the final step and the most often skipped step, yet it is probably the most important step in the process. With this step you can know whether or not you got the correct answer long before your instructor ever looks at it. We verify the answer by plugging the results from the previous steps into the **original** equation. It is very important to plug into the original equation since you may have made a mistake in the very first step that led you to an incorrect answer.

# Example 

$$
\begin{array} {l}
3(x+ 5)  = 2(-6- x) -2x    \\
3x + 15  =  -12 - 2x  - 2x   \\
x = -\frac{27}{7}
\end{array} 

$$

so the solution set  this problem is  : {$-\frac{27}{7}$}
$$
\begin{aligned}3\left(-\frac{27}{7}+5\right)&\overset{?}{\operatorname*{\operatorname*{=}}}2\left(-6-\left(-\frac{27}{7}\right)\right)-2\left(-\frac{27}{7}\right)\\3\left(\frac{8}{7}\right)&\frac{?}{=}2\left(-\frac{15}{7}\right)+\frac{54}{7}\\\frac{24}{7}&=\frac{24}{7}\quad\mathrm{~OK}\end{aligned}
$$

#verify 
plug  $-\frac{27}{7}$ in  we 

$$
\begin{array} {l}
\frac{m-2}{3}  + 1 =   \frac{2m}{7}  \\
21\cdot\frac{m-2}{3}  + 21 =   21\cdot\frac{2m}{7}  \\
7(m-2 ) +  21 =   3\cdot2m \\
7m  -   14   + 21 = 6m  \\
m  = -7  
\end{array} 

$$
so the solution set  this problem is  : {$-7$}
#verify  
![[Pasted image 20250223151349.png]]

$$
\begin{array} {l}
\frac{5}{2y - 6 }  = \frac{10- y}{y^2  - 6y +  9 }    \\
\frac{5}{2(y-3) }  = \frac{10- y}{(y  - 3) (y -3 ) }    \\ 
(y-3)\cdot5  = 2(10- y)   \\
5y  - 15   = 20  - 2y  \\
y  = 5  
\end{array} 

$$
![[Section 2.2 Linear Equations 2025-02-23 15.16.42.excalidraw]]
#verify   
$$\begin{aligned}\frac{5}{2\left(5\right)-6}&\overset{?}{\operatorname*{\operatorname*{\operatorname*{\operatorname*{=}}}}}\frac{10-5}{5^{2}-6\left(5\right)+9}\\\frac{5}{4}&=\frac{5}{4}&\mathrm{OK}\end{aligned}$$


$$
\begin{array} {l}
\frac{2z }{z  + 3 }  = \frac{3}{z-10 }  +  2   \\
(z-10)\cdot 2z = (z  + 3  )\cdot3 +  2\cdot(z  + 3  )(z-10)\\ 
2z^2  - 20z   = 3z   +  9  +  2z^2  -  14z  - 60   \\
z = \frac{51}{9}  \\
 z =  \frac{17}{3}
\end{array} 

$$






$$
\begin{array} {l}
 \frac{2}{x + 2}   = \frac{-x}{ x^2  +5x  + 6}  \\
 \frac{2}{x + 2}     =  \frac{-x}{ (x +  2) (x + 3)} \\
2\cdot (x + 3)  =  -x  \\
x  = -2
\end{array} 
$$
So  , we get a solution in the list of number we need to avoid so we can't get division by  0 and we can't used it  as a solution  . That okay that just mean this equation have no solution 
![[Section 2.2 Linear Equations 2025-02-24 16.15.55.excalidraw]]

$$
\begin{array} {l}
 \frac{2}{x + 1}   = 4 -  \frac{2x}{x+1}  \\
2  = 4(x + 1 ) - 2x\\
2  =4x +  4- 2x   \\
x  = -1 
\end{array} 
$$

So , we arrive  at the single x that we need to avoid . Therefore , this equation have no solution 


#  #Practice_Exercise 

$$
\begin{array} {l}
4x - 7  ( 2 - x )  =  3x  + 2   \\
4x - 14  +  7x  =  3x + 2  \\
8x  = 16   \\
x  = 2 
\end{array}
$$ 

$$
\begin{array} {l}
2(w + 3) - 10  =  6(32 - 3w )   \\
2w  + 6   - 10  =  192  - 18w  \\
20w  =  196   \\
x  =\frac{49}{5}
\end{array}
$$ 
![[Pasted image 20250224163008.png]] 


$$
\begin{array}{l}
\frac{4-2z}{  3}  = \frac{3}{4} -  \frac{5z}{ 6}  \\
4\cdot (4-2z )  =  3\cdot 3  - 2\cdot  5z  \\
16  -  8z  = 9 - 10z   \\
2z   =  -7  \\
z  = -\frac{7}{2} 
\end{array}{}

$$


$$
\begin{array}{l}
\frac{3y + 4 }{ y - 1} = 2  +  \frac{7}{y-1}  \\
3y +4   =  2(y - 1) + 7  \\
3y + 4  = 2y - 2  +  7  \\
y = 1 
\end{array}

$$
So , we arrive at the single z  we need to avoid . Therefore , this solution have no answer 

$$
\begin{array} {l }
\frac{4t}{t^2   -  25}  = \frac{1}{5-t  }  \\
\frac{4t}{(t  - 5) ( t+ 5)   }= \frac{1}{5-t  }   \\
4t  =  -t  - 5   \\
t =  -\frac{5}{5} =   - 1    
\end{array} 
$$From this we can also see that we’ll need to avoid t=5t=5 and t=−5t=−5. Remember that we have to avoid division by zero and we will clearly get division by zero with each of these values of tt.$$
\begin{array} {l }
\frac{5x}{3x  -  3 } + \frac{6}{x + 2 }  = \frac{5}{3}  \\
\frac{5x}{3 (x  -  1) } + \frac{6}{x + 2 }  = \frac{5}{3}  \\
 5x(x + 2 )  +  6\cdot 3(x - 1 )  = (x -1 ) (x + 2  ) 5 \\
5x^2  +  10x  + 18x  -  18  =  (x^2  + 2x  - x  - 2) 5  \\
5x^2  +  10x  + 18x  -  18  =  5x^2 + 10x  - 5x  - 10   \\
   x   =   \frac{8}{23}    
\end{array} 
$$
From this we can also see that we’ll need to avoid x=-2  and  x  =1  a. Remember that we have to avoid division by zero and we will clearly get division by zero with each of these values of xx
