

# #definition 

we will  look at equation  and   inequation  that  contain absolute value .  We  will  look  at equations  with  absolute  value in them  and  look  at inequation in the next chapter
we need to discuss that the  notation for absolute  value is  p  and $\mid p \mid$ note  that the bar for  absolute value is  not parentheses 

##  Geometric Definition 
In this definition  we are going to thing  of  $\mid p \mid$ as  the distance of p from the origin  on the number line   . Also  , we will  always  use a positive value for distance 
 ![[Pasted image 20250320194833.png]] 
 from this  we can get the following  absolute value 
 $$
 \mid  2 \mid  = 2     \;  \mid -3 \mid  = 3  \; \mid \frac{9}{2} \mid    =  \frac{9}{2}
 $$
 
## mathematic Definition  
we can  also  give a strict mathematical  formula   for  definition 

$$
|p| =
\begin{cases}
    p, & \text{if } p \geq 0 \\
    -p, & \text{if } p < 0
\end{cases}
$$
this tell us to drop the absolute  notation for p  if it is  positive , if it negative then add a negative sign  at the beginning 
So  here are a couple of quick example   
$$
\begin{aligned}
    |4| &= 4 \quad &\text{because } 4 \geq 0 \\
    |-8| &= -(-8) = 8 \quad &\text{because } -8 < 0 \\
    |0| &= 0 \quad &\text{because } 0 \geq 0
\end{aligned}
$$
note that we used the same definition  for  geometric interpretation 
one way to think of  absolute value is that it  input  put a  number and make it positive 
$$
\mid p \mid \geq  0  
$$
regardless of the value of    p 

we  need to  be careful to not miss used the definition of this value  .  for example  we cannot used the definition on  
$$\mid -x \mid   $$because  we don't know if x is positive or negative 
don't make the assumption that positive will make all the negative sign  into  positive one   for example   
$$
\mid  4x    -3  \mid     \neq  4x  + 3  
$$
this equation   answer is not true , to prove it let plug in  some number 
$$
7=|−7|=|4(−1)−3|≠4(−1)+3=−1
$$
1.  the two number when  evaluated  are not the same  
2. second the number on the right is negative while the number on  the left is positive  


$$|p|=4$$
Now, if we think of this from a geometric point of view this means that whatever pp is it must have a distance of 4 from the origin. Well there are only two numbers that have a distance of 4 from the origin, namely 4 and -4. So, there are two solutions to this equation,

$$p=−4\;  or\; p=4$$
Now  , if you think of it  we can do  this  for any positive number  not including  4 leading to the following formula  for the equation 
$$If  \; |p|=b,b>0 \;then \;p=−b\;or p=b$$ this only  apply if b is a positive number we will look  at cases where b is negative or  zero 
## solve each of the following equation 

$$\begin{array}{l}
\mid 2x  -  5  \mid   = 9   \\
 \left\{
\begin{array}{l} 
2x  -  5 =  - 9  \\
2x  -  5  =  +   9     \\

\end{array} \\

\right.    
\implies
 \left\{
\begin{array}{l} 
x   =  -2  \\
x  =   7    \\

\end{array} \\

\right.
\end{array} $$$$
\begin{array}{l}
\mid 1-  3t  \mid   =  20   \\
\left\{
\begin{array}{l} 
 1-  3t = 20  \\
 1-  3t = - 20    \\

\end{array} \\

\right.    
\implies
 \left\{
\begin{array}{l} 
x   =  -\frac{19}{3}   \\
x  =   7 \\

\end{array} \\

\right.
\end{array}
$$
$$
\begin{array}{l}
\mid 5y  - 8 \mid  =  1  \\
\left\{
\begin{array}{l} 
5y  - 8 = 1  \\
5y  - 8 = -1    \\

\end{array} \\

\right.    
\implies
 \left\{
\begin{array}{l} 
x   =  \frac{9}{5}  \\
x  =    \frac{7}{5}\\

\end{array} \\

\right.
\end{array}
$$
## where  b is  zero or negative  
$$\begin{array}{l}
\mid 10x−3 \mid   = 0    \\
 \left\{
\begin{array}{l} 
10x    =   3  

\end{array} \\

\right.    
\implies
 \left\{
\begin{array}{l} 
x   =  3

\end{array} \\

\right.
\end{array} $$
here  since the  equation is  0   we can just solve it like  normal 

$$\begin{array}{l}
\mid 15x  + 9  \mid   = -3 \\

\end{array} $$ there is  $|p|≥0$ .  In other word  ,  we cannot get a  negative value out   of the absolute value.  That is  what the equation is saying .   As a result , there  is  **no  solution** to this equation 


##    absolute   values   other than one  real value 

at this  point we have look  at equation that have an absolute number  on the  other side of = sign . However , there are cases where it can  be more than  a number and cases  where it is not a number at all 



$$\begin{array}{l}
|x−2|=3x+1   \\
 \left\{
\begin{array}{l} 
x−2=  - (3x+1) \\
x−2 = 3x+1  \\

\end{array} \\

\right.    
\implies
 \left\{
\begin{array}{l} 
x−2 =   -  3x  +  1 \\
x−2  = 3x+1  \\

\end{array} \\
\right.    
\implies
 \left\{
\begin{array}{l} 
x   =  \frac{1}{4} \\
x   =  -\frac{3}{2} \\

\end{array} \\
\right.
\end{array} $$

note  however that  if we plug  in  the solution  $x  =-\frac{3}{2}$  into the equation it will output this error 
because if we plug it into the equation  
$$
\begin{array}{l}
|-\frac{3}{2} −2|=3\left( -\frac{3}{2} \right)+1      \\
\frac{7}{2      } \neq   -\frac{7}{2}
\end{array}

$$
we will get  a solution on the other side but it is a  negative sign  causing the equation to fail  




$$
\begin{array}{l}
|4x+3|=3−x   \\
\left\{
\begin{array}{l} 
4x+3 =  - (3−x ) \\
4x+3= 3−x   \\

\end{array} \\

\right.    
\implies
 \left\{
\begin{array}{l} 
4x+3  =  -3   +  x  \\
4x+3   = 3−x   \\

\end{array} \\
\right.    
\implies
 \left\{
\begin{array}{l} 
x   = -2 \\
x   =  0 \\

\end{array} \\
\right.
\end{array}

$$
we will get  a solution on the other side but it is a  negative sign  causing the equation to fail  
even  thought  there are  two  solution  there  is not  solution  that  contradict  the equation when  plug  in so  we can take both  solution  x = -2  and  x = 0  





This case looks very different from any of the previous problems we’ve worked to this point and in this case the formula we’ve been using doesn’t really work at all. However, if we think about this a little we can see that we’ll still do something similar here to get a solution.

Both sides of the equation contain absolute values and so the only way the two sides are equal will be if the two quantities inside the absolute value bars are equal or equal but with opposite signs. Or in other words, we must have,


$$
\begin{array}{l}
|2x   - 1 |=|4x+9|   \\
\left\{
\begin{array}{l} 
2x   - 1 =  - (4x+9) \\
2x   - 1 = 4x+9   \\

\end{array} \\

\right.    
\implies
 \left\{
\begin{array}{l} 
2x   - 1 =  - 4x  - 9   \\
2x   - 1 = 4x+9    \\

\end{array} \\
\right.    
\implies
 \left\{
\begin{array}{l} 
x   = \\
x   =  0 \\

\end{array} \\
\right.
\end{array}

$$

Now, we won’t need to verify our solutions here as we did in the previous two parts of this problem. Both with be solutions provided we solved the two equations correctly. However, it will probably be a good idea to verify them anyway just to show that the solution technique we used here really did work properly.

Let’s first check x=−43x=−43.

∣∣∣2(−43)−1∣∣∣?=∣∣∣4(−43)+9∣∣∣∣∣∣−113∣∣∣?=∣∣∣113∣∣∣113=113OK|2(−43)−1|=?⁡|4(−43)+9||−113|=?⁡|113|113=113OK

In the case the quantities inside the absolute value were the same number but opposite signs. However, upon taking the absolute value we got the same number and so x=−43x=−43 is a solution. Now, let’s check x=−5x=−5.

|2(−5)−1|?=|4(−5)+9||−11|?=|−11|11=11OK|2(−5)−1|=?⁡|4(−5)+9||−11|=?⁡|−11|11=11OK

In the case we got the same value inside the absolute value bars.

So, as suggested above both answers did in fact work and both are solutions to the equation.