# Show that each of the following numbers are solutions to the given equation or inequality.

$$
\begin{array}{l}
x =3  \; in \;  x^2   - 9   =  0  \\ \\
(x+ 3 ) (x-3 ) =  0   \\
\{\begin{array}\{
x =  -3   \\
x = + 3
\end{array}
\end{array}

 $$
We first plug the proposed solution into the equation.
 $$
 \begin{aligned}3^2-9&\overset{?}{\operatorname*{\operatorname*{=}}}0\\9-9&=0\\0&=0&\mathrm{OK}\end{aligned}
 $$
 
So, what we are asking here is does the right side equal the left side after we plug in the proposed solution. That is the meaning of the “?” above the equal sign in the first line.

Since the right side and the left side are the same we say that x=3x=3 **satisfies** the equation. 




$$
\begin{array}{l}
 x = 3  \;   in  \;  3(y +1 )   =  4y  -5   \\
3y  + 3    - 4y  +  5   = 0   \\
-y  + 8  = 0   \\
y  = 8  
\end{array}
$$ So, we want to see if y=8y=8 satisfies the equation. First plug the value into the equation.
$$
\begin{aligned}3\left(8+1\right)&\overset{?}{\operatorname*{\operatorname*{=}}}4\left(8\right)-5\\27&=27\quad\mathrm{OK}\\\\\end{aligned}$$
So, y=8y=8 satisfies the equation and so is a solution.




$$
\begin{array} {l}
z =1    \;  in \;   2(z - 5 )  \leq 4 \\
2z -10   \leq 4  \\
z  \leq  7 
\end{array}
$$

In this case we’ve got an inequality and in this case “satisfy” means something slightly different. In this case we will say that a number will satisfy the inequality if, after plugging it in, we get a true inequality as a result. 
Let’s check z=1.
$$
\begin{aligned}2\left(1-5\right)&\overset{?}{\operatorname*{\operatorname*{\operatorname*{\operatorname*{\leq}}}}}4\left(1\right)\\-8&\leq4\quad\mathrm{OK}\end{aligned}
$$

So, -8 is less than or equal to 4 (in fact it’s less than) and so we have a true inequality. Therefore z=1z=1 will satisfy the inequality and hence is a solution 



$$
\begin{array}{l}
z=-5 \; in \;  2(z-5) \leq  4z \\
2z - 10  \leq 4z  \\
z  \leq 7   
\end{array}
$$This is the same inequality with a different value so let’s check that.

$$
\begin{aligned}2\left(-5-5\right)&\overset{?}{\operatorname*{\operatorname*{\operatorname*{\operatorname*{\leq}}}}}4\left(-5\right)\\-20&\leq-20\quad\mathrm{OK}\end{aligned}
$$
In this case -20 is less than or equal to -20 (in this case it’s equal) and so again we get a true inequality and so z=−5z=−5 satisfies the inequality and so will be a solution.



# Show that the following number aren't solution  to the given equation or inequality 
In this case we do essentially the same thing that we did in the previous example. Plug the number in and show that this time it doesn’t satisfy the equation. For equations that will mean that the right side of the equation will not equal the left side of the equation.
$$
\begin{array} {l}
y  =  -2  \;  in  \; 3(y+ 1)  = 4y-5  \\
3y +  3  = 4y - 5   \\
y = -8
\end{array} 
$$
$$
\begin{aligned}3\left(-2+1\right)&\overset{?}{\operatorname*{\operatorname*{\operatorname*{=}}}}4\left(-2\right)-5\\-3&\neq-13\mathrm{~NOT~OK}\end{aligned}

$$

So, -3 is not the same as -13 and so the equation isn’t satisfied. Therefore y=−2y=−2 isn’t a solution to the equation.



This time we’ve got an inequality. A number will not satisfy an inequality if we get an inequality that isn’t true after plugging the number in. 
$$

\begin{aligned}2\left(-12-5\right)&\overset{?}{\operatorname*{\operatorname*{\operatorname*{\operatorname*{\leq}}}}}4\left(-12\right)\\-34&\overset{\searrow}{\operatorname*{\operatorname*{\operatorname*{\operatorname*{\leq}}}}}-48\mathrm{~NOT~OK}\end{aligned}
$$



$$
\begin{array} {l}

z=  -12  \;  in  \;  2(z-5)  \leq  4z  \\
2z  - 10  \leq 4z   \\
z  \geq -5 
\end{array} 
$$
In this case -34 is NOT less than or equal to -48 and so the inequality isn’t satisfied. Therefore z=−12z=−12 is not a solution to the inequality.


# #definition  
now there is no reason to think that  the given equation and inequality will have only one solution . Look at the single 