---
title: Adjunction
date: 2025-02-05
references: https://www.youtube.com/watch?v=qgwjhfjCvJ4&list=PLC292123722B1B450&index=10
tags:
  - In_Progress
reference:
---

A FRACTION WHERE BOTH THE NUMER AND DENOM. ARE  POLYNOMIALS 
$$\frac{P}{Q}$$
 ex :  $$
 \frac{P}{Q}
 $$
 ex    
 $$
\frac{5x  -3}{2} \; \frac{x^2 - 1}{x + 1}  \;  \frac{13}{x^2  - 5x  + 6 }
 $$

$$
f(x)   = \frac{x-3}{x^3}
$$
- this is a rational  function  \
- you can never divide by 0  in a rational function  

Note : for any rational function the denominator   cannot be zero   
if the denominator is zero at some point then the function is zero at that point 
it okay for a numerator to equal to zero 

$$
f(x) =  \frac{x^2   + 1  }{x-6}
$$
find domains  : number  
$$


\{\begin{array}{l}
x |  is \;  A \; real \; number  \cap x \neq 6 
\end{array}


$$
- not okey due to the rule the denominator is not a real number 
- $x - 6  \neq 0 \implies x   = 6$ 
To Find Domain  , Set Denominator $\neq$ 0 


$G(x) = \frac{x^2+ 9}{4}$
$$


\{\begin{array}{l}
x |  is \;  A \; real \; number    
\end{array}


$$

$$h(x) =  \frac{5x^2 + 9}{x+ 2}$$$$
\{\begin{array}{l}
x |  is \;  A \; real \; number   \cap x \neq -2  
\end{array}
$$- $x + 2  \neq 0 \implies x   = -2$



$$f(x) =  \frac{5x + 4}{x^2 - 3x - 10}$$ 

$$
\{\begin{array}{l}
x |  is \;  A \; real \; number    \cap x \neq 5   , x  \neq -2 
\end{array}
$$ $x^2 - 3x - 10   \neq 0$  
![[Rational Function 2025-02-07 17.29.18.excalidraw]] 
$$
\begin{aligned}
(x-5)(x+ 2 )\neq 0  \\
\{\begin{array}{l}
x-5 \neq 0   \\
x+ 2 \neq 0  \\

\end{array} 
\{\begin{array}{l}
x \neq5\\
x \neq - 2 \\

\end{array}
\end{aligned}

$$ 
# simplify  
$$
\begin{array}{l}
\frac{5}{17}  \\
\frac{6}{18} 
\end{array} 
$$
simplify when the denominator and  numerator is similar have common value 
Faction 

$$\frac{15}{35}  =  \frac{5\cdot 3}{ 5\cdot 7 }  = \frac{5}{  5 } \cdot \frac{3}{  7   }  = \frac{3}{7}$$

the first thing  you need to do before  common factor you need to know factoring  
$$
\begin{array}{l}
\frac{(x+2)^2}{x^2 - 4}  \\
=\frac{(x+2)^2}{x^2 - 2^2}  \\
=\frac{(x+2)^2}{(x-2 )(x+ 2)} \\
=\frac{(x+2)}{(x-2 )} \\
\end{array} $$
$$ \begin{array}{l}
\frac{3y^3}{6y^4  - 3y^3}  \\
 = \frac{3y^3}{3y^3 (2y -1)} \\
= \frac{1}{2y - 1}
\end{array}
$$

$$
\frac{5x^2 -6x + 1}{ 3x^2 + 4x- 7} 
$$

![[7.1 Rational Function 2025-02-10 13.20.34.excalidraw]]

![[7.1 Rational Function 2025-02-10 13.21.00.excalidraw]]
$$ 
\begin{array}{l}
\frac{5x^2 -6x + 1}{ 3x^2 + 4x- 7}    \\
 = \frac{5x^2 -6x + 1}{ 3x^2 + 4x- 7}  \\
 = \frac{(3x + 7)(x -1 )}{ ( 5x- 1)(x -1 )}  \\
 = \frac{(3x + 7)}{ ( 5x- 1)}
\end{array} 

$$

$$ 
\begin{array}{l}
\frac{5x^4}{ 10x^5  -  5z^3 }    \\
 = \frac{5x^4}{ 5x^3\cdot(2x^2 - 1 ) }   \\
 = \frac{x}{ 2x^2 - 1 }  \\
\end{array} 

$$
Factor  to make the term with the largest exponent positive   
Step: 
1. Factor both numerator and denominator completely    
2. Simplify  Common factor , not common terms  
HTTP://sites.google.com/site/professorleon57  for home work 
$$
\begin{array}{l} 
\frac{20-5x^2}{x^2 + x - 6}   \\
= \frac{-5(-4 + x^2)}{(x+3)(x - 2)}   \\
 = \frac{-5(x^2 - 4)}{(x+3)(x - 2)}   \\
 = \frac{-5\cdot(x - 2 ) (x+ 2)}{(x+3)(x - 2)}   \\
 = \frac{-5(x+ 2)}{(x+3)} 
\end{array} 

$$


$$
\begin{array}{l}
\frac{9x^5  - 3x^4}{ 3x^3}  \\
=\frac{3x^3(3x^2  - 1x)}{ 3x^3 }  \\   \\
= 3x^2  - x 
\end{array}
$$ 



$$
\begin{array}{l}
\frac{3 -  3x^2}{ x^2 + x - 2}  \\
=\frac{-3( x^2  - 1)}{  }  \\ 
= 3x^2  - x 
\end{array}
$$ 