

step :  
1. factor completely 
2. write as 1 fraction 
3. simplify 

$$ 
\begin{array}{l}
\frac{7}{5 }  \\
= \frac{7}{5 }  \frac{15}{11}    \\
 = \frac{105}{55}  
\end{array}
$$ 


$$ 
\begin{array}{l}
\frac{7}{5 }  \\
= \frac{7}{5 }  \frac{15}{11}    \\ 
 = \frac{105}{55}  
\end{array}
$$


or 
$$ 
\begin{array}{l}
\frac{7}{5 }  \\
= \frac{7}{5 }  \frac{15}{11}    \\ 
= \frac{7}{1}  \frac{3}{11}    \\   \\
= \frac{21}{11}  
\end{array}
$$

ex

$$ 
\begin{array}{l}
\frac{- 5x^3  }{3b^3}  \cdot \frac{2b^2 }{15x}    \\
 = \frac{- 5x^3\cdot2b^2 }{3b^3\cdot 15x}    \\
=   \frac{2x^2  }{9b}   
\end{array}
$$ 

$$ 
\begin{array}{l}
\frac{3x^4    }{2y^3}  \cdot \frac{y^2 }{-9x^5}    \\
 = \frac{3x^4  \cdot2y^3 }{y^2\cdot -9x^5}    \\
=   \frac{2y }{ -3x}  
\end{array}
$$ 
$$
\begin{array}{l}
 \frac{6x +  6}{7}\cdot  \frac{14}{x^2 -1 }  \\
   = \frac{6x +  6}{7}\cdot  \frac{14}{x^2 -1 }    \\
 = \frac{6(x+ 1) 14 }{7}\cdot  \frac{14}{(x - 1) ( x+ 1) }  \\
 = \frac{6}{1}\cdot  \frac{2}{(x - 1)  }   \\
 = \frac{12}{(x - 1)}
\end{array}
$$ $$
\begin{array}{l}
\frac{x^2  -x }{ 5x  }  . \frac{15}{x^2  -1  } \\
=\frac{x(x -1 ) \cdot 15 }{ 5x (x  - 1) (x + 1) }    \\
=\frac{ 15 }{ 5(x+ 1)  }   \\
=\frac{ 3 }{ (x+ 1)  }  
\end{array}
$$ 


$$ 
\begin{array}{l}
 \frac{4x + 8}{14x - 7x^2 }  \cdot  \frac{3x^2 - 5x - 2}{9x^2 -1 }    \\  \\
 \frac{4(x+ 2)}{-7(x +  2) }  \cdot  \frac{(x -2) (x + 3 )}{9x^2 -1 }  \\ 
 \frac{(4x + 8)\cdot (3x^2 - 5x - 2 )}{(14x - 7x^2)(3x^2 -1) } 
\end{array}
$$ 
![[7.2 Multi and Division  RAT Expressions 2025-02-10 15.22.13.excalidraw]]

 $$
\begin{array}{l}
 
\end{array}
$$

 



