---
title: Adjunction
date: 2025-02-05
references: https://www.youtube.com/watch?v=cuyPbznFD9o&list=PLC292123722B1B450&indey=5
tags:
  - In_Progress
reference:
---

Note when you have an equation with the power of 2 (quadrative) move everything to one side  , a on the left and 0 on the right of = 
Zero  product  properties  
$a.b = 0$    
$a = 0   \; or \; b = 0$  
Exercise  
 $(y+1)(y-3)   = 0$
$$

\left\{
\begin{array}{l}
y + 1 = 0  \\
y-3 = 0   \\

\end{array}
\right.
\implies
\left\{
\begin{array}{l}
y  = - 1   \\
y = +3  \\

\end{array}
\right.

$$


$$
\begin{array}
 & y^2 -3y  -18 =  0   \\
(y-6)(y+3)  =   0  
\end{array}
$$

$$


\left\{
\begin{array}{l}
y  -  6 = 0  \\
y + 3 = 0   \\

\end{array}
\right.
\implies
\left\{
\begin{array}{l}
y  = 6 \\
y =  - 3  \\

\end{array}
\right.

$$  


$$
\begin{array}
 & y^2 + 5y  + 6  =  0   \\
(y+3)(y+2)  =   0  
\end{array}
$$

$$


\left\{
\begin{array}{l}
y  + 2 = 0  \\
y + 3 = 0   \\

\end{array}
\right.
\implies
\left\{
\begin{array}{l}
y  = -2 \\
y =  - 3  \\

\end{array}
\right.

$$  



$$
\begin{array}
 & 25y^2 - 29y  + 4  =  0    
 \\ 25y(y-1)-4y(y-1) =    0   \\
(25y-4y)(y-1) =    0  \\


\end{array}
$$

$$


\left\{
\begin{array}{l}
y  -1  = 0  \\
25y  - 4 = 0   \\

\end{array}
\right.
\implies
\left\{
\begin{array}{l}
y  = 1 \\
y =  \frac{4}{25}  \\

\end{array}
\right.

$$  




$$
\begin{array}
 & y(y -4 ) =  5      
 \\  y(y -4 )     - 5 =    0   \\
y^2 -  4y      - 5 =    0  \\ 
(y - 5)(y +1) =   0  \\


\end{array}
$$

$$


\left\{
\begin{array}{l}
y  + 1  = 0  \\
y-5  = 0   \\

\end{array}
\right.
\implies
\left\{
\begin{array}{l}
y  =  - 1 \\
y =  5  \\

\end{array}
\right.

$$




$$
\begin{array}
 & (3y - 2 ) ( 2y^2    -13 y  + 15 ) =  0    
 \\ (3y - 2 ) (y+1) ( 2y  -15 )   =    0   \\


\end{array}
$$

$$


\left\{
\begin{array}{l}
3y  -2  = 0  \\
2y - 15  = 0   \\
y  +1  = 0  \\

\end{array}
\right.
\implies
\left\{
\begin{array}{l}
y   = \frac{2}{3}  \\
y   = -1  \\
y   = \frac{15}{2}  \\
\end{array}
\right.

$$  


