---
title: Adjunction
date: <% tp.date.now("YYYY-MM-DD") %>
references: 
tags:
  - In_Progress
reference:
---


[asdfds](https://tutorial.math.lamar.edu/Problems/Alg/IntegerExponents.aspx)

# definition
##   Polynomial in one variable  
Polynomial in one variable is  algebraic expression that  consist of term like  
$ax^n$ 
- a being a real number and is call the coefficient of the term 
- n being a positive  integer number 
- x being the place holder variable 
The degree in the polynomial is the call the largest exponent in the polynomial  
 A **monomial** is a polynomial that consists of exactly one term. A **binomial** is a polynomial that consists of exactly two terms. Finally, a **trinomial** is a polynomial that consists of exactly three terms. We will use these terms off and on so you should probably be at least somewhat familiar with them.
### example 
$$\begin{aligned}&5x^{12}-2x^6+x^5-198x+1&&\mathrm{degree}:12\\&x^4-x^3+x^2-x+1&&\mathrm{degree}:4\\&56x^{23}&&\mathrm{degree}:23\\&5x-7&&\mathrm{degree}:1\\&-8&&\mathrm{degree}:0\end{aligned}$$
we can see that a polynomial can consist of  a single term  with the bottom three equation  
in the last equation -8 even thought  it seem to not resemble a polynomial it can be rewritten as $-8x^0$ 
### example of non polynomials
$$
\begin{aligned}&4x^6+15x^{-8}+1\\&5\sqrt{x}-x+x^2\\&\frac2x+x^3-2\end{aligned}
$$
- the first equation is not a polynomial  due to the fact that there is a negative exponent  
- the second equation is not a polynomial due to the fact that it have  a factorial exponent and all exponent need to be integer 
- the third equation have a negative exponent -1 if you convert $\frac{2}{x} = 2x^{-1}$   all exponent need to be positive 

## polynomial in two variable 
polynomial in two variable are algebraic expression  consisting of term  in the form  of  $ax^{n}y^{m}$ 
the degree of a two variable polynomial is the highest sum of the exponent in each term  
$$
\begin{gathered}
x^2y-6x^3y^{12}+10x^2-7y+1 \text{degree} \text{:15} \\
6x^4+8y^4-xy^2 \text{degree} \text{:4} \\
x^4y^2-x^3y^3-xy+x^4 \text{degree} \text{:6} \\
6x^{14}-10y^3+3x-11y \text{degree} \text{:14} 
\end{gathered}
$$


## solving equation  by factoring 

Note when you have an equation with the power of 2 (quadrative) move everything to one side  , a on the left and 0 on the right of = 
Zero  product  properties  
$a.b = 0$    
$a = 0   \; or \; b = 0$  
$(y+1)(y-3)   = 0$
$$

\left\{
\begin{array}{l}
y + 1 = 0  \\
y-3 = 0   \\

\end{array}
\right.
\implies
\left\{
\begin{array}{l}
y  = - 1   \\
y = +3  \\

\end{array}
\right.

$$ 
# formula  
$$
(3x+5)(3x-5) =  9x^2  -15x  + 15x  -25 =  9x^2  - 25
$$
$$
(2x+6)^2   =   4x^2 +  24x + 36   
$$
$$
(1-7x)^2  =  49x^2 -14x + 1 
$$
$$
4(x+3)^2 =  4(x^2 + 6x +9)  =  4x^2 + 24x +  36 
$$
## Different of Squares 
$$
(a+b) (a-b)   =  a^2   - b^2 
$$

## Square of Sum 
$$
(a+b)^2 =  a^2  - 2ab + b^2
$$

## Square of a Different 

$$
(a-b)^2 =  a^2  - 2ab +b^2  
$$

# Practice  Exercise 
## multiplication  of  number 
$4x^2.(x^2-6x+2)= 4x^4 -24x^3 +8x^2$

## used the FOIL method for multiplying the binomial 
![[Pasted image 20241201195150.png]]
the FOIL method just mean that we are multiplying the first every turn in this first binomial with every term in the second binomial 
$(3x +5).(x-10)=3x^2-30+5x-50=3x^2-25-50$

$\left(4x^2-x\right)(6-3x)=24x^2-12x^3-6x+3x^2=-12x^3+27x^2-6x$
$$
(2x+3 )(x^2-x +1) =  2x^3 - 2x^2 +2x +3x^2 -3X+3= 2X^3 +X^2 -X +3 
$$
