---
title: Adjunction
date: 2024-11-20-14:45:50-04:00
references: 
tags:
  - In_Progress
reference:
---
# definition 
Rational exponents is a more complicated from of simple exponent. Instead of looking at exponents as simply integer Rational exponents add in a new layer of depth with the used of faction in the form of 
$$
 b^{m/n}
$$

# additional Rational exponents principle with integer exponents 

we should also know that the properties of [[Integer Exponents]] can still be apply  to rational exponents  
$$
(a^n)^m =  a^{n \cdot{m}}
$$

if we saw something in it radical form we can see it in it exponent form  :  
$$
\sqrt[4]{ 5 }^7 =  5^{7/4} 
$$
$$
\sqrt[b]{a }  =  x^{a/b} =  x^{a \cdot{1/b}}
$$

the exponent with the fraction of  $a^{c/b}$ will be equal to $a^{c \cdot{1/b} }$ 
in other word radical exponent is a combination of a integer number and a fractional number 

# special cases 
$a=  b^{1/n}$ is equivalent to  $a^{n} = b$ 
in  this cases  we are asking the question of what number n so that a can be equal to b or in reverses what square root of n do we need to get a 

an example 
$$
4   = \sqrt[2]{ 16 }
$$
so the square root of 16 is the value of 4 
will combine the special cases radical exponent with the [[Integer Exponents]] product properties  

# practice exercise  

##  Evaluate each of the following

1. $$
25^{1/2} =  \sqrt{ 25 } =  5 
 $$
 2. $$
32^{1/5}=  \sqrt[5]{32  } =  2
$$
3. $$
81^{1/4} = (81^{1/2})^{1/2} = 3
$$
4. $$
(-8)^{1/3} =  -2 
$$
5. $$
(-16)^{1/4}
$$
- this question have no answer do to the rule  
- $a=  b^{1/n}$ is equivalent to  $a^{n} = b$  
- no number raise by a even power can be negative 
6. $$
 -16^{1/4}  =  -(16^{1/4}) = -(2) = -2
$$

- In the situation above, the negative sign is excluded from the  root operation. Without parentheses, the exponent applies only to the number 16 , not to the negative sign 

## simply  each of the following 

$$
\begin{aligned}&\left(\frac{x^{2}y^{-2/3}}{x^{\frac{1}{2}}y^{-3}}\right)^{-\frac{1}{7}}=\left(x^{2},x^{1/2}y^{-2/3}y^{3}\right)^{-1/7}\\&=\left(x^{5/2},y^{7/3}\right)^{-1/7}=x^{-5/14},y^{-1/3}\\&\frac{1}{x^{5/14}y^{1/3}}\end{aligned}
$$
**instructor answer**
$$
 \left(\frac{x^2y^{-\frac23}}{x^{-\frac12}y^{-3}}\right)^{-\frac17}=\frac1{\left(x^{\frac52}y^{\frac73}\right)^{\frac17}}=\frac1{x^{\frac5{14}}y^{\frac13}}
$$
- here the instructor used the properties  7 to remove any negative number and then used properties 4 to clean up the equation 
- the instructor used the properties [[Integer Exponents#7. Negative Exponent Rule for Multiplication]] to remove any negative power exponents then used [[Integer Exponents#4. Distributive Rule of Exponents over Multiplication]] to clean up the equation  
#  practice exercise


$$
\left( \frac{9}{4} \right)^{1/2}  =  \frac{3}{4}
$$
$$
\left( \frac{8}{343} \right)^{-2/3}= \left( \frac{2}{7} \right)^{-2} = \left( \frac{49}{4} \right)
$$

## simplify the equation 
$$
(a^3 .b^{-1/4})^{2/3} =  a^2 . b^{-1/6} = \frac{a^2}{b^{1/6}}
$$
$$
x^{1/4} . x^{-1/5} =  x^{1/20}
$$$$
\left( \frac{q^3.p^{-1/2}}{q^{-1/3}.p} \right)^{3/7}  =  \left( \frac{q^3.q^{1/3}}{p^{1/2}.p} \right)^{3/7} = \left( \frac{q^{10/3}}{p^{3/2}} \right)^{3/7} = \frac{q^{10/7}}{p^{9/14}}
$$
$$
\begin{aligned}&\left(\frac{m^{\frac12}n^{-\frac13}}{n^{\frac23}m^{-\frac74}}\right)^{-\frac16}=\left(\frac{m^{\frac12}m^{\frac74}}{n^{\frac23}n^{\frac13}}\right)^{-\frac16}=\left(\frac{m^{\frac94}}{n^1}\right)^{-\frac16}=\left(\frac n{m^{\frac94}}\right)^{\frac16}=\boxed{\frac{n^{\frac16}}{m^{\frac38}}}\\&\bullet\end{aligned}
$$
## rationalize the denominator. Assume that xx and yy are both positive.  
rationalize mean    
$-\frac{6}{\sqrt{ 5x }+10\sqrt{ y }}$  
multiply the [[faction#definition]] numerator and denominator by conjugate 
= $-\frac{(6.\sqrt{ 5x }-60\sqrt{ y })}{(\sqrt{ 5x }+10\sqrt{ y }).(\sqrt{ 5x }-10\sqrt{ y })}$ 
=$-\frac{(6.\sqrt{ 5x }-60\sqrt{ y })}{( 5x +10\sqrt{ y }.\sqrt{ 5x } - 10\sqrt{ y }.\sqrt{ 5x } +  100y)}$ 
= $-\frac{(6.\sqrt{ 5x }-60\sqrt{ y })}{( 5x +  100y)}$ 
